minimal working backend w/o GC implementation

benchmarks/fibonacci/extraction/CertiCoq.Benchmarks.Fibonacci.fib.program.c
@@ -1,0 +1,1690 @@
+#ifndef CERTICOQ_BENCHMARKS_FIBONACCI_FIB_PROGRAM_C
+#define CERTICOQ_BENCHMARKS_FIBONACCI_FIB_PROGRAM_C
+#include <gc_stack.h>
+#include <prim_string.h>
+#include <prim_floats.h>
+#include <prim_int63.h>
+#include <coq_c_ffi.h>
+#include "CertiCoq.Benchmarks.Fibonacci.fib.program.h"
+extern struct thread_info *make_tinfo(void);
+extern value f_case_known_123(struct thread_info *, value, value);
+extern value succ_known_122(struct thread_info *, value);
+extern value of_succ_nat_known_121(struct thread_info *, value);
+extern value f_case_known_120(struct thread_info *, value);
+extern value fib_loop_nat_uncurried_uncurried_known_119(struct thread_info *, value, value, value);
+extern value iter_uncurried_known_118(struct thread_info *, value, value);
+extern value f_case_known_117(struct thread_info *, value);
+extern value f_case_known_116(struct thread_info *, value);
+extern value to_Z_rec_uncurried_known_115(struct thread_info *, value, value);
+extern value CoqdZArithdBinIntDefdZdsucc_double_wrapper_114(struct thread_info *, value, value);
+extern value pred_double_known_113(struct thread_info *, value);
+extern value CoqdZArithdBinIntDefdZdsucc_double_known_112(struct thread_info *, value);
+extern value CoqdZArithdBinIntDefdZddouble_wrapper_111(struct thread_info *, value, value);
+extern value CoqdZArithdBinIntDefdZddouble_known_110(struct thread_info *, value);
+extern value add_uncurried_known_109(struct thread_info *, value, value);
+extern value of_pos_rec_uncurried_known_108(struct thread_info *, value, value);
+extern value body(struct thread_info *);
+value f_case_known_123(struct thread_info *, value, value);
+value succ_known_122(struct thread_info *, value);
+value of_succ_nat_known_121(struct thread_info *, value);
+value f_case_known_120(struct thread_info *, value);
+value fib_loop_nat_uncurried_uncurried_known_119(struct thread_info *, value, value, value);
+value iter_uncurried_known_118(struct thread_info *, value, value);
+value f_case_known_117(struct thread_info *, value);
+value f_case_known_116(struct thread_info *, value);
+value to_Z_rec_uncurried_known_115(struct thread_info *, value, value);
+value CoqdZArithdBinIntDefdZdsucc_double_wrapper_114(struct thread_info *, value, value);
+value pred_double_known_113(struct thread_info *, value);
+value CoqdZArithdBinIntDefdZdsucc_double_known_112(struct thread_info *, value);
+value CoqdZArithdBinIntDefdZddouble_wrapper_111(struct thread_info *, value, value);
+value CoqdZArithdBinIntDefdZddouble_known_110(struct thread_info *, value);
+value add_uncurried_known_109(struct thread_info *, value, value);
+value of_pos_rec_uncurried_known_108(struct thread_info *, value, value);
+value body(struct thread_info *);
+unsigned long long const body_info_356[2] = { 126LL, 0LL, };
+
+unsigned long long const of_pos_rec_uncurried_known_info_355[4] = { 0LL, 2LL,
+  0LL, 1LL, };
+
+unsigned long long const add_uncurried_known_info_354[4] = { 0LL, 2LL, 0LL,
+  1LL, };
+
+unsigned long long const CoqdZArithdBinIntDefdZddouble_known_info_353[3] = {
+  4LL, 1LL, 0LL, };
+
+unsigned long long const CoqdZArithdBinIntDefdZddouble_wrapper_info_352[4] = {
+  0LL, 2LL, 0LL, 1LL, };
+
+unsigned long long const CoqdZArithdBinIntDefdZdsucc_double_known_info_351[3] = {
+  4LL, 1LL, 0LL, };
+
+unsigned long long const pred_double_known_info_350[3] = { 4LL, 1LL, 0LL, };
+
+unsigned long long const CoqdZArithdBinIntDefdZdsucc_double_wrapper_info_349[4] = {
+  0LL, 2LL, 0LL, 1LL, };
+
+unsigned long long const to_Z_rec_uncurried_known_info_348[4] = { 0LL, 2LL,
+  0LL, 1LL, };
+
+unsigned long long const f_case_known_info_347[3] = { 3LL, 1LL, 0LL, };
+
+unsigned long long const f_case_known_info_346[3] = { 2LL, 1LL, 0LL, };
+
+unsigned long long const iter_uncurried_known_info_345[4] = { 0LL, 2LL, 0LL,
+  1LL, };
+
+unsigned long long const fib_loop_nat_uncurried_uncurried_known_info_344[5] = {
+  0LL, 3LL, 0LL, 1LL, 2LL, };
+
+unsigned long long const f_case_known_info_343[3] = { 0LL, 1LL, 0LL, };
+
+unsigned long long const of_succ_nat_known_info_342[3] = { 0LL, 1LL, 0LL, };
+
+unsigned long long const succ_known_info_341[3] = { 2LL, 1LL, 0LL, };
+
+unsigned long long const f_case_known_info_340[4] = { 0LL, 2LL, 0LL, 1LL, };
+
+value f_case_known_123(struct thread_info *$tinfo, value $s_252, value $CoqdNumbersdCyclicdInt63dUint63dsize_253)
+{
+  struct stack_frame frame;
+  value root[2];
+  register value $y_254;
+  register value $p_255;
+  register value $p_257;
+  register value $y_259;
+  register value $y_260;
+  register value $prim_261;
+  register value *$alloc;
+  register value *$limit;
+  register value *$args;
+  register _Bool $arg;
+  register value $result;
+  $alloc = (*$tinfo).alloc;
+  $limit = (*$tinfo).limit;
+  $args = (*$tinfo).args;
+  frame.next = root;
+  frame.root = root;
+  frame.prev = (*$tinfo).fp;
+  if (($s_252 & 1) == 0) {
+    switch (*((value *) $s_252 + -1LL) & 255LL) {
+      case 0:
+        $p_255 = *((value *) $s_252 + 0LL);
+        $args = (*$tinfo).args;
+        (*$tinfo).alloc = $alloc;
+        (*$tinfo).limit = $limit;
+        $result =
+          ((value (*)(struct thread_info *, value, value)) of_pos_rec_uncurried_known_108)
+          ($tinfo, $p_255, $CoqdNumbersdCyclicdInt63dUint63dsize_253);
+        return $result;
+        break;
+      default:
+        $p_257 = *((value *) $s_252 + 0LL);
+        $args = (*$tinfo).args;
+        (*$tinfo).alloc = $alloc;
+        (*$tinfo).limit = $limit;
+        /*skip*/;
+        $y_259 =
+          ((value (*)(struct thread_info *, value, value)) of_pos_rec_uncurried_known_108)
+          ($tinfo, $p_257, $CoqdNumbersdCyclicdInt63dUint63dsize_253);
+        $alloc = (*$tinfo).alloc;
+        $limit = (*$tinfo).limit;
+        /*skip*/;
+        $y_260 = 1LLU;
+        $prim_261 =
+          ((value (*)(value, value)) prim_int63_sub)
+          ($y_260, $y_259);
+        (*$tinfo).alloc = $alloc;
+        (*$tinfo).limit = $limit;
+        return $prim_261;
+        break;
+      
+    }
+  } else {
+    switch ($s_252 >> 1LL) {
+      default:
+        $y_254 = 1LLU;
+        (*$tinfo).alloc = $alloc;
+        (*$tinfo).limit = $limit;
+        return $y_254;
+        break;
+      
+    }
+  }
+}
+
+value succ_known_122(struct thread_info *$tinfo, value $x_243)
+{
+  struct stack_frame frame;
+  value root[1];
+  register value $p_244;
+  register value $y_245;
+  register value $y_246;
+  register value $p_247;
+  register value $y_248;
+  register value $y_249;
+  register value $y_250;
+  register value *$alloc;
+  register value *$limit;
+  register value *$args;
+  register _Bool $arg;
+  register value $result;
+  $alloc = (*$tinfo).alloc;
+  $limit = (*$tinfo).limit;
+  $args = (*$tinfo).args;
+  frame.next = root;
+  frame.root = root;
+  frame.prev = (*$tinfo).fp;
+  if (!(2LL <= $limit - $alloc)) {
+    *(root + 0LL) = $x_243;
+    frame.next = root + 1LL;
+    (*$tinfo).fp = &frame;
+    (*$tinfo).nalloc = 2LL;
+    garbage_collect($tinfo);
+    $x_243 = *(root + 0LL);
+    (*$tinfo).fp = frame.prev;
+    $alloc = (*$tinfo).alloc;
+    $limit = (*$tinfo).limit;
+  }
+  if (($x_243 & 1) == 0) {
+    switch (*((value *) $x_243 + -1LL) & 255LL) {
+      case 0:
+        $p_244 = *((value *) $x_243 + 0LL);
+        $args = (*$tinfo).args;
+        (*$tinfo).alloc = $alloc;
+        (*$tinfo).limit = $limit;
+        /*skip*/;
+        $y_245 =
+          ((value (*)(struct thread_info *, value)) succ_known_122)
+          ($tinfo, $p_244);
+        $alloc = (*$tinfo).alloc;
+        $limit = (*$tinfo).limit;
+        if (!(2LL <= $limit - $alloc)) {
+          *(root + 0LL) = $y_245;
+          frame.next = root + 1LL;
+          (*$tinfo).fp = &frame;
+          (*$tinfo).nalloc = 2LL;
+          garbage_collect($tinfo);
+          $y_245 = *(root + 0LL);
+          (*$tinfo).fp = frame.prev;
+          $alloc = (*$tinfo).alloc;
+          $limit = (*$tinfo).limit;
+        }
+        /*skip*/;
+        $y_246 = (value) ($alloc + 1LL);
+        $alloc = $alloc + 2LL;
+        *((value *) $y_246 + -1LL) = 1025LL;
+        *((value *) $y_246 + 0LL) = $y_245;
+        (*$tinfo).alloc = $alloc;
+        (*$tinfo).limit = $limit;
+        return $y_246;
+        break;
+      default:
+        $p_247 = *((value *) $x_243 + 0LL);
+        $y_248 = (value) ($alloc + 1LL);
+        $alloc = $alloc + 2LL;
+        *((value *) $y_248 + -1LL) = 1024LL;
+        *((value *) $y_248 + 0LL) = $p_247;
+        (*$tinfo).alloc = $alloc;
+        (*$tinfo).limit = $limit;
+        return $y_248;
+        break;
+      
+    }
+  } else {
+    switch ($x_243 >> 1LL) {
+      default:
+        $y_249 = 1LL;
+        $y_250 = (value) ($alloc + 1LL);
+        $alloc = $alloc + 2LL;
+        *((value *) $y_250 + -1LL) = 1025LL;
+        *((value *) $y_250 + 0LL) = $y_249;
+        (*$tinfo).alloc = $alloc;
+        (*$tinfo).limit = $limit;
+        return $y_250;
+        break;
+      
+    }
+  }
+}
+
+value of_succ_nat_known_121(struct thread_info *$tinfo, value $n_237)
+{
+  struct stack_frame frame;
+  value root[1];
+  register value $y_238;
+  register value $x_239;
+  register value $y_240;
+  register value *$alloc;
+  register value *$limit;
+  register value *$args;
+  register _Bool $arg;
+  register value $result;
+  $alloc = (*$tinfo).alloc;
+  $limit = (*$tinfo).limit;
+  $args = (*$tinfo).args;
+  frame.next = root;
+  frame.root = root;
+  frame.prev = (*$tinfo).fp;
+  if (($n_237 & 1) == 0) {
+    switch (*((value *) $n_237 + -1LL) & 255LL) {
+      default:
+        $x_239 = *((value *) $n_237 + 0LL);
+        $args = (*$tinfo).args;
+        (*$tinfo).alloc = $alloc;
+        (*$tinfo).limit = $limit;
+        /*skip*/;
+        $y_240 =
+          ((value (*)(struct thread_info *, value)) of_succ_nat_known_121)
+          ($tinfo, $x_239);
+        $alloc = (*$tinfo).alloc;
+        $limit = (*$tinfo).limit;
+        /*skip*/;
+        $args = (*$tinfo).args;
+        (*$tinfo).alloc = $alloc;
+        (*$tinfo).limit = $limit;
+        $result =
+          ((value (*)(struct thread_info *, value)) succ_known_122)
+          ($tinfo, $y_240);
+        return $result;
+        break;
+      
+    }
+  } else {
+    switch ($n_237 >> 1LL) {
+      default:
+        $y_238 = 1LL;
+        (*$tinfo).alloc = $alloc;
+        (*$tinfo).limit = $limit;
+        return $y_238;
+        break;
+      
+    }
+  }
+}
+
+value f_case_known_120(struct thread_info *$tinfo, value $s_230)
+{
+  struct stack_frame frame;
+  value root[1];
+  register value $y_231;
+  register value $n_232;
+  register value $y_234;
+  register value $y_235;
+  register value *$alloc;
+  register value *$limit;
+  register value *$args;
+  register _Bool $arg;
+  register value $result;
+  $alloc = (*$tinfo).alloc;
+  $limit = (*$tinfo).limit;
+  $args = (*$tinfo).args;
+  frame.next = root;
+  frame.root = root;
+  frame.prev = (*$tinfo).fp;
+  if (($s_230 & 1) == 0) {
+    switch (*((value *) $s_230 + -1LL) & 255LL) {
+      default:
+        $n_232 = *((value *) $s_230 + 0LL);
+        $args = (*$tinfo).args;
+        (*$tinfo).alloc = $alloc;
+        (*$tinfo).limit = $limit;
+        /*skip*/;
+        $y_234 =
+          ((value (*)(struct thread_info *, value)) of_succ_nat_known_121)
+          ($tinfo, $n_232);
+        $alloc = (*$tinfo).alloc;
+        $limit = (*$tinfo).limit;
+        if (!(2LL <= $limit - $alloc)) {
+          *(root + 0LL) = $y_234;
+          frame.next = root + 1LL;
+          (*$tinfo).fp = &frame;
+          (*$tinfo).nalloc = 2LL;
+          garbage_collect($tinfo);
+          $y_234 = *(root + 0LL);
+          (*$tinfo).fp = frame.prev;
+          $alloc = (*$tinfo).alloc;
+          $limit = (*$tinfo).limit;
+        }
+        /*skip*/;
+        $y_235 = (value) ($alloc + 1LL);
+        $alloc = $alloc + 2LL;
+        *((value *) $y_235 + -1LL) = 1024LL;
+        *((value *) $y_235 + 0LL) = $y_234;
+        (*$tinfo).alloc = $alloc;
+        (*$tinfo).limit = $limit;
+        return $y_235;
+        break;
+      
+    }
+  } else {
+    switch ($s_230 >> 1LL) {
+      default:
+        $y_231 = 1LL;
+        (*$tinfo).alloc = $alloc;
+        (*$tinfo).limit = $limit;
+        return $y_231;
+        break;
+      
+    }
+  }
+}
+
+value fib_loop_nat_uncurried_uncurried_known_119(struct thread_info *$tinfo, value $b_223, value $a_224, value $i_225)
+{
+  struct stack_frame frame;
+  value root[3];
+  register value $ip_226;
+  register value $y_228;
+  register value *$alloc;
+  register value *$limit;
+  register value *$args;
+  register _Bool $arg;
+  register value $result;
+  $alloc = (*$tinfo).alloc;
+  $limit = (*$tinfo).limit;
+  $args = (*$tinfo).args;
+  frame.next = root;
+  frame.root = root;
+  frame.prev = (*$tinfo).fp;
+  if (($i_225 & 1) == 0) {
+    switch (*((value *) $i_225 + -1LL) & 255LL) {
+      default:
+        $ip_226 = *((value *) $i_225 + 0LL);
+        $args = (*$tinfo).args;
+        (*$tinfo).alloc = $alloc;
+        (*$tinfo).limit = $limit;
+        *(root + 1LL) = $ip_226;
+        *(root + 0LL) = $a_224;
+        frame.next = root + 2LL;
+        (*$tinfo).fp = &frame;
+        $y_228 =
+          ((value (*)(struct thread_info *, value, value)) add_uncurried_known_109)
+          ($tinfo, $b_223, $a_224);
+        $alloc = (*$tinfo).alloc;
+        $limit = (*$tinfo).limit;
+        $ip_226 = *(root + 1LL);
+        $a_224 = *(root + 0LL);
+        (*$tinfo).fp = frame.prev;
+        $args = (*$tinfo).args;
+        (*$tinfo).alloc = $alloc;
+        (*$tinfo).limit = $limit;
+        $result =
+          ((value (*)(struct thread_info *, value, value, value)) fib_loop_nat_uncurried_uncurried_known_119)
+          ($tinfo, $a_224, $y_228, $ip_226);
+        return $result;
+        break;
+      
+    }
+  } else {
+    switch ($i_225 >> 1LL) {
+      default:
+        (*$tinfo).alloc = $alloc;
+        (*$tinfo).limit = $limit;
+        return $b_223;
+        break;
+      
+    }
+  }
+}
+
+value iter_uncurried_known_118(struct thread_info *$tinfo, value $a_212, value $p_213)
+{
+  struct stack_frame frame;
+  value root[2];
+  register value $p_214;
+  register value $y_216;
+  register value $y_217;
+  register value $p_219;
+  register value $y_221;
+  register value *$alloc;
+  register value *$limit;
+  register value *$args;
+  register _Bool $arg;
+  register value $result;
+  $alloc = (*$tinfo).alloc;
+  $limit = (*$tinfo).limit;
+  $args = (*$tinfo).args;
+  frame.next = root;
+  frame.root = root;
+  frame.prev = (*$tinfo).fp;
+  if (($p_213 & 1) == 0) {
+    switch (*((value *) $p_213 + -1LL) & 255LL) {
+      case 0:
+        $p_214 = *((value *) $p_213 + 0LL);
+        $args = (*$tinfo).args;
+        (*$tinfo).alloc = $alloc;
+        (*$tinfo).limit = $limit;
+        *(root + 1LL) = $p_214;
+        *(root + 0LL) = $a_212;
+        frame.next = root + 2LL;
+        (*$tinfo).fp = &frame;
+        $y_216 =
+          ((value (*)(struct thread_info *, value, value)) add_uncurried_known_109)
+          ($tinfo, $a_212, $a_212);
+        $alloc = (*$tinfo).alloc;
+        $limit = (*$tinfo).limit;
+        $p_214 = *(root + 1LL);
+        $a_212 = *(root + 0LL);
+        (*$tinfo).fp = frame.prev;
+        $args = (*$tinfo).args;
+        (*$tinfo).alloc = $alloc;
+        (*$tinfo).limit = $limit;
+        *(root + 0LL) = $a_212;
+        frame.next = root + 1LL;
+        (*$tinfo).fp = &frame;
+        $y_217 =
+          ((value (*)(struct thread_info *, value, value)) iter_uncurried_known_118)
+          ($tinfo, $y_216, $p_214);
+        $alloc = (*$tinfo).alloc;
+        $limit = (*$tinfo).limit;
+        $a_212 = *(root + 0LL);
+        (*$tinfo).fp = frame.prev;
+        $args = (*$tinfo).args;
+        (*$tinfo).alloc = $alloc;
+        (*$tinfo).limit = $limit;
+        $result =
+          ((value (*)(struct thread_info *, value, value)) add_uncurried_known_109)
+          ($tinfo, $y_217, $a_212);
+        return $result;
+        break;
+      default:
+        $p_219 = *((value *) $p_213 + 0LL);
+        $args = (*$tinfo).args;
+        (*$tinfo).alloc = $alloc;
+        (*$tinfo).limit = $limit;
+        *(root + 0LL) = $p_219;
+        frame.next = root + 1LL;
+        (*$tinfo).fp = &frame;
+        $y_221 =
+          ((value (*)(struct thread_info *, value, value)) add_uncurried_known_109)
+          ($tinfo, $a_212, $a_212);
+        $alloc = (*$tinfo).alloc;
+        $limit = (*$tinfo).limit;
+        $p_219 = *(root + 0LL);
+        (*$tinfo).fp = frame.prev;
+        $args = (*$tinfo).args;
+        (*$tinfo).alloc = $alloc;
+        (*$tinfo).limit = $limit;
+        $result =
+          ((value (*)(struct thread_info *, value, value)) iter_uncurried_known_118)
+          ($tinfo, $y_221, $p_219);
+        return $result;
+        break;
+      
+    }
+  } else {
+    switch ($p_213 >> 1LL) {
+      default:
+        (*$tinfo).alloc = $alloc;
+        (*$tinfo).limit = $limit;
+        return $a_212;
+        break;
+      
+    }
+  }
+}
+
+value f_case_known_117(struct thread_info *$tinfo, value $s_204)
+{
+  struct stack_frame frame;
+  value root[1];
+  register value $y_205;
+  register value $p_206;
+  register value $y_208;
+  register value $y_209;
+  register value $y_210;
+  register value *$alloc;
+  register value *$limit;
+  register value *$args;
+  register _Bool $arg;
+  register value $result;
+  $alloc = (*$tinfo).alloc;
+  $limit = (*$tinfo).limit;
+  $args = (*$tinfo).args;
+  frame.next = root;
+  frame.root = root;
+  frame.prev = (*$tinfo).fp;
+  if (!(2LL <= $limit - $alloc)) {
+    *(root + 0LL) = $s_204;
+    frame.next = root + 1LL;
+    (*$tinfo).fp = &frame;
+    (*$tinfo).nalloc = 2LL;
+    garbage_collect($tinfo);
+    $s_204 = *(root + 0LL);
+    (*$tinfo).fp = frame.prev;
+    $alloc = (*$tinfo).alloc;
+    $limit = (*$tinfo).limit;
+  }
+  if (($s_204 & 1) == 0) {
+    switch (*((value *) $s_204 + -1LL) & 255LL) {
+      case 0:
+        $p_206 = *((value *) $s_204 + 0LL);
+        $y_208 = 1LL;
+        $y_209 = (value) ($alloc + 1LL);
+        $alloc = $alloc + 2LL;
+        *((value *) $y_209 + -1LL) = 1024LL;
+        *((value *) $y_209 + 0LL) = $y_208;
+        $args = (*$tinfo).args;
+        (*$tinfo).alloc = $alloc;
+        (*$tinfo).limit = $limit;
+        $result =
+          ((value (*)(struct thread_info *, value, value)) iter_uncurried_known_118)
+          ($tinfo, $y_209, $p_206);
+        return $result;
+        break;
+      default:
+        $y_210 = 1LL;
+        (*$tinfo).alloc = $alloc;
+        (*$tinfo).limit = $limit;
+        return $y_210;
+        break;
+      
+    }
+  } else {
+    switch ($s_204 >> 1LL) {
+      default:
+        $y_205 = 1LL;
+        (*$tinfo).alloc = $alloc;
+        (*$tinfo).limit = $limit;
+        return $y_205;
+        break;
+      
+    }
+  }
+}
+
+value f_case_known_116(struct thread_info *$tinfo, value $s_198)
+{
+  struct stack_frame frame;
+  value root[1];
+  register value $CoqdZArithdBinIntDefdZdsucc_double_wrapperbogus_env_199;
+  register value $CoqdZArithdBinIntDefdZdsucc_double_wrapper_clo_200;
+  register value $CoqdZArithdBinIntDefdZddouble_wrapperbogus_env_201;
+  register value $CoqdZArithdBinIntDefdZddouble_wrapper_clo_202;
+  register value *$alloc;
+  register value *$limit;
+  register value *$args;
+  register _Bool $arg;
+  register value $result;
+  $alloc = (*$tinfo).alloc;
+  $limit = (*$tinfo).limit;
+  $args = (*$tinfo).args;
+  frame.next = root;
+  frame.root = root;
+  frame.prev = (*$tinfo).fp;
+  if (!(3LL <= $limit - $alloc)) {
+    *(root + 0LL) = $s_198;
+    frame.next = root + 1LL;
+    (*$tinfo).fp = &frame;
+    (*$tinfo).nalloc = 3LL;
+    garbage_collect($tinfo);
+    $s_198 = *(root + 0LL);
+    (*$tinfo).fp = frame.prev;
+    $alloc = (*$tinfo).alloc;
+    $limit = (*$tinfo).limit;
+  }
+  if (($s_198 & 1) == 0) {
+    switch (*((value *) $s_198 + -1LL) & 255LL) {
+      
+    }
+  } else {
+    switch ($s_198 >> 1LL) {
+      case 0:
+        $CoqdZArithdBinIntDefdZdsucc_double_wrapperbogus_env_199 = 1LL;
+        $CoqdZArithdBinIntDefdZdsucc_double_wrapper_clo_200 =
+          (value) ($alloc + 1LL);
+        $alloc = $alloc + 3LL;
+        *((value *) $CoqdZArithdBinIntDefdZdsucc_double_wrapper_clo_200
+           + -1LL) =
+          2048LL;
+        *((value *) $CoqdZArithdBinIntDefdZdsucc_double_wrapper_clo_200
+           + 0LL) =
+          CoqdZArithdBinIntDefdZdsucc_double_wrapper_114;
+        *((value *) $CoqdZArithdBinIntDefdZdsucc_double_wrapper_clo_200
+           + 1LL) =
+          $CoqdZArithdBinIntDefdZdsucc_double_wrapperbogus_env_199;
+        (*$tinfo).alloc = $alloc;
+        (*$tinfo).limit = $limit;
+        return $CoqdZArithdBinIntDefdZdsucc_double_wrapper_clo_200;
+        break;
+      default:
+        $CoqdZArithdBinIntDefdZddouble_wrapperbogus_env_201 = 1LL;
+        $CoqdZArithdBinIntDefdZddouble_wrapper_clo_202 =
+          (value) ($alloc + 1LL);
+        $alloc = $alloc + 3LL;
+        *((value *) $CoqdZArithdBinIntDefdZddouble_wrapper_clo_202 + -1LL) =
+          2048LL;
+        *((value *) $CoqdZArithdBinIntDefdZddouble_wrapper_clo_202 + 0LL) =
+          CoqdZArithdBinIntDefdZddouble_wrapper_111;
+        *((value *) $CoqdZArithdBinIntDefdZddouble_wrapper_clo_202 + 1LL) =
+          $CoqdZArithdBinIntDefdZddouble_wrapperbogus_env_201;
+        (*$tinfo).alloc = $alloc;
+        (*$tinfo).limit = $limit;
+        return $CoqdZArithdBinIntDefdZddouble_wrapper_clo_202;
+        break;
+      
+    }
+  }
+}
+
+value to_Z_rec_uncurried_known_115(struct thread_info *$tinfo, value $i_182, value $n_183)
+{
+  struct stack_frame frame;
+  value root[2];
+  register value $y_184;
+  register value $n_185;
+  register value $y_187;
+  register value $prim_188;
+  register value $y_189;
+  register value $prim_190;
+  register value $y_191;
+  register value $y_192;
+  register value $prim_193;
+  register value $y_194;
+  register value $y_code_195;
+  register value $y_env_196;
+  register value *$alloc;
+  register value *$limit;
+  register value *$args;
+  register _Bool $arg;
+  register value $result;
+  $alloc = (*$tinfo).alloc;
+  $limit = (*$tinfo).limit;
+  $args = (*$tinfo).args;
+  frame.next = root;
+  frame.root = root;
+  frame.prev = (*$tinfo).fp;
+  if (($n_183 & 1) == 0) {
+    switch (*((value *) $n_183 + -1LL) & 255LL) {
+      default:
+        $n_185 = *((value *) $n_183 + 0LL);
+        $y_187 = 3LLU;
+        $prim_188 =
+          ((value (*)(value, value)) prim_int63_land)
+          ($i_182, $y_187);
+        $y_189 = 1LLU;
+        $prim_190 =
+          ((value (*)(value, value)) prim_int63_eqb)
+          ($prim_188, $y_189);
+        $args = (*$tinfo).args;
+        (*$tinfo).alloc = $alloc;
+        (*$tinfo).limit = $limit;
+        *(root + 1LL) = $n_185;
+        *(root + 0LL) = $i_182;
+        frame.next = root + 2LL;
+        (*$tinfo).fp = &frame;
+        $y_191 =
+          ((value (*)(struct thread_info *, value)) f_case_known_116)
+          ($tinfo, $prim_190);
+        $alloc = (*$tinfo).alloc;
+        $limit = (*$tinfo).limit;
+        $n_185 = *(root + 1LL);
+        $i_182 = *(root + 0LL);
+        (*$tinfo).fp = frame.prev;
+        $y_192 = 3LLU;
+        $prim_193 =
+          ((value (*)(value, value)) prim_int63_lsr)
+          ($i_182, $y_192);
+        $args = (*$tinfo).args;
+        (*$tinfo).alloc = $alloc;
+        (*$tinfo).limit = $limit;
+        *(root + 0LL) = $y_191;
+        frame.next = root + 1LL;
+        (*$tinfo).fp = &frame;
+        $y_194 =
+          ((value (*)(struct thread_info *, value, value)) to_Z_rec_uncurried_known_115)
+          ($tinfo, $prim_193, $n_185);
+        $alloc = (*$tinfo).alloc;
+        $limit = (*$tinfo).limit;
+        $y_191 = *(root + 0LL);
+        (*$tinfo).fp = frame.prev;
+        $y_code_195 = *((value *) $y_191 + 0LL);
+        $y_env_196 = *((value *) $y_191 + 1LL);
+        $args = (*$tinfo).args;
+        (*$tinfo).alloc = $alloc;
+        (*$tinfo).limit = $limit;
+        $result =
+          ((value (*)(struct thread_info *, value, value)) $y_code_195)
+          ($tinfo, $y_env_196, $y_194);
+        return $result;
+        break;
+      
+    }
+  } else {
+    switch ($n_183 >> 1LL) {
+      default:
+        $y_184 = 1LL;
+        (*$tinfo).alloc = $alloc;
+        (*$tinfo).limit = $limit;
+        return $y_184;
+        break;
+      
+    }
+  }
+}
+
+value CoqdZArithdBinIntDefdZdsucc_double_wrapper_114(struct thread_info *$tinfo, value $env_178, value $x_179)
+{
+  struct stack_frame frame;
+  value root[1];
+  register value *$alloc;
+  register value *$limit;
+  register value *$args;
+  register _Bool $arg;
+  register value $result;
+  $alloc = (*$tinfo).alloc;
+  $limit = (*$tinfo).limit;
+  $args = (*$tinfo).args;
+  frame.next = root;
+  frame.root = root;
+  frame.prev = (*$tinfo).fp;
+  $args = (*$tinfo).args;
+  (*$tinfo).alloc = $alloc;
+  (*$tinfo).limit = $limit;
+  $result =
+    ((value (*)(struct thread_info *, value)) CoqdZArithdBinIntDefdZdsucc_double_known_112)
+    ($tinfo, $x_179);
+  return $result;
+}
+
+value pred_double_known_113(struct thread_info *$tinfo, value $x_170)
+{
+  struct stack_frame frame;
+  value root[1];
+  register value $p_171;
+  register value $y_172;
+  register value $y_173;
+  register value $p_174;
+  register value $y_175;
+  register value $y_176;
+  register value $y_177;
+  register value *$alloc;
+  register value *$limit;
+  register value *$args;
+  register _Bool $arg;
+  register value $result;
+  $alloc = (*$tinfo).alloc;
+  $limit = (*$tinfo).limit;
+  $args = (*$tinfo).args;
+  frame.next = root;
+  frame.root = root;
+  frame.prev = (*$tinfo).fp;
+  if (!(4LL <= $limit - $alloc)) {
+    *(root + 0LL) = $x_170;
+    frame.next = root + 1LL;
+    (*$tinfo).fp = &frame;
+    (*$tinfo).nalloc = 4LL;
+    garbage_collect($tinfo);
+    $x_170 = *(root + 0LL);
+    (*$tinfo).fp = frame.prev;
+    $alloc = (*$tinfo).alloc;
+    $limit = (*$tinfo).limit;
+  }
+  if (($x_170 & 1) == 0) {
+    switch (*((value *) $x_170 + -1LL) & 255LL) {
+      case 0:
+        $p_171 = *((value *) $x_170 + 0LL);
+        $y_172 = (value) ($alloc + 1LL);
+        $alloc = $alloc + 2LL;
+        *((value *) $y_172 + -1LL) = 1025LL;
+        *((value *) $y_172 + 0LL) = $p_171;
+        $y_173 = (value) ($alloc + 1LL);
+        $alloc = $alloc + 2LL;
+        *((value *) $y_173 + -1LL) = 1024LL;
+        *((value *) $y_173 + 0LL) = $y_172;
+        (*$tinfo).alloc = $alloc;
+        (*$tinfo).limit = $limit;
+        return $y_173;
+        break;
+      default:
+        $p_174 = *((value *) $x_170 + 0LL);
+        $args = (*$tinfo).args;
+        (*$tinfo).alloc = $alloc;
+        (*$tinfo).limit = $limit;
+        /*skip*/;
+        $y_175 =
+          ((value (*)(struct thread_info *, value)) pred_double_known_113)
+          ($tinfo, $p_174);
+        $alloc = (*$tinfo).alloc;
+        $limit = (*$tinfo).limit;
+        if (!(2LL <= $limit - $alloc)) {
+          *(root + 0LL) = $y_175;
+          frame.next = root + 1LL;
+          (*$tinfo).fp = &frame;
+          (*$tinfo).nalloc = 2LL;
+          garbage_collect($tinfo);
+          $y_175 = *(root + 0LL);
+          (*$tinfo).fp = frame.prev;
+          $alloc = (*$tinfo).alloc;
+          $limit = (*$tinfo).limit;
+        }
+        /*skip*/;
+        $y_176 = (value) ($alloc + 1LL);
+        $alloc = $alloc + 2LL;
+        *((value *) $y_176 + -1LL) = 1024LL;
+        *((value *) $y_176 + 0LL) = $y_175;
+        (*$tinfo).alloc = $alloc;
+        (*$tinfo).limit = $limit;
+        return $y_176;
+        break;
+      
+    }
+  } else {
+    switch ($x_170 >> 1LL) {
+      default:
+        $y_177 = 1LL;
+        (*$tinfo).alloc = $alloc;
+        (*$tinfo).limit = $limit;
+        return $y_177;
+        break;
+      
+    }
+  }
+}
+
+value CoqdZArithdBinIntDefdZdsucc_double_known_112(struct thread_info *$tinfo, value $x_159)
+{
+  struct stack_frame frame;
+  value root[1];
+  register value $y_160;
+  register value $y_161;
+  register value $p_162;
+  register value $y_163;
+  register value $y_164;
+  register value $p_165;
+  register value $y_167;
+  register value $y_168;
+  register value *$alloc;
+  register value *$limit;
+  register value *$args;
+  register _Bool $arg;
+  register value $result;
+  $alloc = (*$tinfo).alloc;
+  $limit = (*$tinfo).limit;
+  $args = (*$tinfo).args;
+  frame.next = root;
+  frame.root = root;
+  frame.prev = (*$tinfo).fp;
+  if (!(4LL <= $limit - $alloc)) {
+    *(root + 0LL) = $x_159;
+    frame.next = root + 1LL;
+    (*$tinfo).fp = &frame;
+    (*$tinfo).nalloc = 4LL;
+    garbage_collect($tinfo);
+    $x_159 = *(root + 0LL);
+    (*$tinfo).fp = frame.prev;
+    $alloc = (*$tinfo).alloc;
+    $limit = (*$tinfo).limit;
+  }
+  if (($x_159 & 1) == 0) {
+    switch (*((value *) $x_159 + -1LL) & 255LL) {
+      case 0:
+        $p_162 = *((value *) $x_159 + 0LL);
+        $y_163 = (value) ($alloc + 1LL);
+        $alloc = $alloc + 2LL;
+        *((value *) $y_163 + -1LL) = 1024LL;
+        *((value *) $y_163 + 0LL) = $p_162;
+        $y_164 = (value) ($alloc + 1LL);
+        $alloc = $alloc + 2LL;
+        *((value *) $y_164 + -1LL) = 1024LL;
+        *((value *) $y_164 + 0LL) = $y_163;
+        (*$tinfo).alloc = $alloc;
+        (*$tinfo).limit = $limit;
+        return $y_164;
+        break;
+      default:
+        $p_165 = *((value *) $x_159 + 0LL);
+        $args = (*$tinfo).args;
+        (*$tinfo).alloc = $alloc;
+        (*$tinfo).limit = $limit;
+        /*skip*/;
+        $y_167 =
+          ((value (*)(struct thread_info *, value)) pred_double_known_113)
+          ($tinfo, $p_165);
+        $alloc = (*$tinfo).alloc;
+        $limit = (*$tinfo).limit;
+        if (!(2LL <= $limit - $alloc)) {
+          *(root + 0LL) = $y_167;
+          frame.next = root + 1LL;
+          (*$tinfo).fp = &frame;
+          (*$tinfo).nalloc = 2LL;
+          garbage_collect($tinfo);
+          $y_167 = *(root + 0LL);
+          (*$tinfo).fp = frame.prev;
+          $alloc = (*$tinfo).alloc;
+          $limit = (*$tinfo).limit;
+        }
+        /*skip*/;
+        $y_168 = (value) ($alloc + 1LL);
+        $alloc = $alloc + 2LL;
+        *((value *) $y_168 + -1LL) = 1025LL;
+        *((value *) $y_168 + 0LL) = $y_167;
+        (*$tinfo).alloc = $alloc;
+        (*$tinfo).limit = $limit;
+        return $y_168;
+        break;
+      
+    }
+  } else {
+    switch ($x_159 >> 1LL) {
+      default:
+        $y_160 = 1LL;
+        $y_161 = (value) ($alloc + 1LL);
+        $alloc = $alloc + 2LL;
+        *((value *) $y_161 + -1LL) = 1024LL;
+        *((value *) $y_161 + 0LL) = $y_160;
+        (*$tinfo).alloc = $alloc;
+        (*$tinfo).limit = $limit;
+        return $y_161;
+        break;
+      
+    }
+  }
+}
+
+value CoqdZArithdBinIntDefdZddouble_wrapper_111(struct thread_info *$tinfo, value $env_155, value $x_156)
+{
+  struct stack_frame frame;
+  value root[1];
+  register value *$alloc;
+  register value *$limit;
+  register value *$args;
+  register _Bool $arg;
+  register value $result;
+  $alloc = (*$tinfo).alloc;
+  $limit = (*$tinfo).limit;
+  $args = (*$tinfo).args;
+  frame.next = root;
+  frame.root = root;
+  frame.prev = (*$tinfo).fp;
+  $args = (*$tinfo).args;
+  (*$tinfo).alloc = $alloc;
+  (*$tinfo).limit = $limit;
+  $result =
+    ((value (*)(struct thread_info *, value)) CoqdZArithdBinIntDefdZddouble_known_110)
+    ($tinfo, $x_156);
+  return $result;
+}
+
+value CoqdZArithdBinIntDefdZddouble_known_110(struct thread_info *$tinfo, value $x_147)
+{
+  struct stack_frame frame;
+  value root[1];
+  register value $y_148;
+  register value $p_149;
+  register value $y_150;
+  register value $y_151;
+  register value $p_152;
+  register value $y_153;
+  register value $y_154;
+  register value *$alloc;
+  register value *$limit;
+  register value *$args;
+  register _Bool $arg;
+  register value $result;
+  $alloc = (*$tinfo).alloc;
+  $limit = (*$tinfo).limit;
+  $args = (*$tinfo).args;
+  frame.next = root;
+  frame.root = root;
+  frame.prev = (*$tinfo).fp;
+  if (!(4LL <= $limit - $alloc)) {
+    *(root + 0LL) = $x_147;
+    frame.next = root + 1LL;
+    (*$tinfo).fp = &frame;
+    (*$tinfo).nalloc = 4LL;
+    garbage_collect($tinfo);
+    $x_147 = *(root + 0LL);
+    (*$tinfo).fp = frame.prev;
+    $alloc = (*$tinfo).alloc;
+    $limit = (*$tinfo).limit;
+  }
+  if (($x_147 & 1) == 0) {
+    switch (*((value *) $x_147 + -1LL) & 255LL) {
+      case 0:
+        $p_149 = *((value *) $x_147 + 0LL);
+        $y_150 = (value) ($alloc + 1LL);
+        $alloc = $alloc + 2LL;
+        *((value *) $y_150 + -1LL) = 1025LL;
+        *((value *) $y_150 + 0LL) = $p_149;
+        $y_151 = (value) ($alloc + 1LL);
+        $alloc = $alloc + 2LL;
+        *((value *) $y_151 + -1LL) = 1024LL;
+        *((value *) $y_151 + 0LL) = $y_150;
+        (*$tinfo).alloc = $alloc;
+        (*$tinfo).limit = $limit;
+        return $y_151;
+        break;
+      default:
+        $p_152 = *((value *) $x_147 + 0LL);
+        $y_153 = (value) ($alloc + 1LL);
+        $alloc = $alloc + 2LL;
+        *((value *) $y_153 + -1LL) = 1025LL;
+        *((value *) $y_153 + 0LL) = $p_152;
+        $y_154 = (value) ($alloc + 1LL);
+        $alloc = $alloc + 2LL;
+        *((value *) $y_154 + -1LL) = 1025LL;
+        *((value *) $y_154 + 0LL) = $y_153;
+        (*$tinfo).alloc = $alloc;
+        (*$tinfo).limit = $limit;
+        return $y_154;
+        break;
+      
+    }
+  } else {
+    switch ($x_147 >> 1LL) {
+      default:
+        $y_148 = 1LL;
+        (*$tinfo).alloc = $alloc;
+        (*$tinfo).limit = $limit;
+        return $y_148;
+        break;
+      
+    }
+  }
+}
+
+value add_uncurried_known_109(struct thread_info *$tinfo, value $m_141, value $n_142)
+{
+  struct stack_frame frame;
+  value root[2];
+  register value $p_143;
+  register value $y_144;
+  register value $y_145;
+  register value *$alloc;
+  register value *$limit;
+  register value *$args;
+  register _Bool $arg;
+  register value $result;
+  $alloc = (*$tinfo).alloc;
+  $limit = (*$tinfo).limit;
+  $args = (*$tinfo).args;
+  frame.next = root;
+  frame.root = root;
+  frame.prev = (*$tinfo).fp;
+  if (($n_142 & 1) == 0) {
+    switch (*((value *) $n_142 + -1LL) & 255LL) {
+      default:
+        $p_143 = *((value *) $n_142 + 0LL);
+        $args = (*$tinfo).args;
+        (*$tinfo).alloc = $alloc;
+        (*$tinfo).limit = $limit;
+        /*skip*/;
+        $y_144 =
+          ((value (*)(struct thread_info *, value, value)) add_uncurried_known_109)
+          ($tinfo, $m_141, $p_143);
+        $alloc = (*$tinfo).alloc;
+        $limit = (*$tinfo).limit;
+        if (!(2LL <= $limit - $alloc)) {
+          *(root + 0LL) = $y_144;
+          frame.next = root + 1LL;
+          (*$tinfo).fp = &frame;
+          (*$tinfo).nalloc = 2LL;
+          garbage_collect($tinfo);
+          $y_144 = *(root + 0LL);
+          (*$tinfo).fp = frame.prev;
+          $alloc = (*$tinfo).alloc;
+          $limit = (*$tinfo).limit;
+        }
+        /*skip*/;
+        $y_145 = (value) ($alloc + 1LL);
+        $alloc = $alloc + 2LL;
+        *((value *) $y_145 + -1LL) = 1024LL;
+        *((value *) $y_145 + 0LL) = $y_144;
+        (*$tinfo).alloc = $alloc;
+        (*$tinfo).limit = $limit;
+        return $y_145;
+        break;
+      
+    }
+  } else {
+    switch ($n_142 >> 1LL) {
+      default:
+        (*$tinfo).alloc = $alloc;
+        (*$tinfo).limit = $limit;
+        return $m_141;
+        break;
+      
+    }
+  }
+}
+
+value of_pos_rec_uncurried_known_108(struct thread_info *$tinfo, value $p_125, value $n_126)
+{
+  struct stack_frame frame;
+  value root[2];
+  register value $y_127;
+  register value $n_128;
+  register value $p_129;
+  register value $y_130;
+  register value $y_131;
+  register value $prim_132;
+  register value $y_133;
+  register value $prim_134;
+  register value $p_135;
+  register value $y_136;
+  register value $y_137;
+  register value $prim_138;
+  register value $y_139;
+  register value *$alloc;
+  register value *$limit;
+  register value *$args;
+  register _Bool $arg;
+  register value $result;
+  $alloc = (*$tinfo).alloc;
+  $limit = (*$tinfo).limit;
+  $args = (*$tinfo).args;
+  frame.next = root;
+  frame.root = root;
+  frame.prev = (*$tinfo).fp;
+  if (($n_126 & 1) == 0) {
+    switch (*((value *) $n_126 + -1LL) & 255LL) {
+      default:
+        $n_128 = *((value *) $n_126 + 0LL);
+        if (($p_125 & 1) == 0) {
+          switch (*((value *) $p_125 + -1LL) & 255LL) {
+            case 0:
+              $p_129 = *((value *) $p_125 + 0LL);
+              $args = (*$tinfo).args;
+              (*$tinfo).alloc = $alloc;
+              (*$tinfo).limit = $limit;
+              /*skip*/;
+              $y_130 =
+                ((value (*)(struct thread_info *, value, value)) of_pos_rec_uncurried_known_108)
+                ($tinfo, $p_129, $n_128);
+              $alloc = (*$tinfo).alloc;
+              $limit = (*$tinfo).limit;
+              /*skip*/;
+              $y_131 = 3LLU;
+              $prim_132 =
+                ((value (*)(value, value)) prim_int63_lsl)
+                ($y_130, $y_131);
+              $y_133 = 3LLU;
+              $prim_134 =
+                ((value (*)(value, value)) prim_int63_lor)
+                ($prim_132, $y_133);
+              (*$tinfo).alloc = $alloc;
+              (*$tinfo).limit = $limit;
+              return $prim_134;
+              break;
+            default:
+              $p_135 = *((value *) $p_125 + 0LL);
+              $args = (*$tinfo).args;
+              (*$tinfo).alloc = $alloc;
+              (*$tinfo).limit = $limit;
+              /*skip*/;
+              $y_136 =
+                ((value (*)(struct thread_info *, value, value)) of_pos_rec_uncurried_known_108)
+                ($tinfo, $p_135, $n_128);
+              $alloc = (*$tinfo).alloc;
+              $limit = (*$tinfo).limit;
+              /*skip*/;
+              $y_137 = 3LLU;
+              $prim_138 =
+                ((value (*)(value, value)) prim_int63_lsl)
+                ($y_136, $y_137);
+              (*$tinfo).alloc = $alloc;
+              (*$tinfo).limit = $limit;
+              return $prim_138;
+              break;
+            
+          }
+        } else {
+          switch ($p_125 >> 1LL) {
+            default:
+              $y_139 = 3LLU;
+              (*$tinfo).alloc = $alloc;
+              (*$tinfo).limit = $limit;
+              return $y_139;
+              break;
+            
+          }
+        }
+        break;
+      
+    }
+  } else {
+    switch ($n_126 >> 1LL) {
+      default:
+        $y_127 = 1LLU;
+        (*$tinfo).alloc = $alloc;
+        (*$tinfo).limit = $limit;
+        return $y_127;
+        break;
+      
+    }
+  }
+}
+
+value body(struct thread_info *$tinfo)
+{
+  struct stack_frame frame;
+  value root[2];
+  register value $y_262;
+  register value $y_263;
+  register value $y_264;
+  register value $y_265;
+  register value $y_266;
+  register value $y_267;
+  register value $y_268;
+  register value $y_269;
+  register value $y_270;
+  register value $y_271;
+  register value $y_272;
+  register value $y_273;
+  register value $y_274;
+  register value $y_275;
+  register value $y_276;
+  register value $y_277;
+  register value $y_278;
+  register value $y_279;
+  register value $y_280;
+  register value $y_281;
+  register value $y_282;
+  register value $y_283;
+  register value $y_284;
+  register value $y_285;
+  register value $y_286;
+  register value $y_287;
+  register value $y_288;
+  register value $y_289;
+  register value $y_290;
+  register value $y_291;
+  register value $y_292;
+  register value $y_293;
+  register value $y_294;
+  register value $y_295;
+  register value $y_296;
+  register value $y_297;
+  register value $y_298;
+  register value $y_299;
+  register value $y_300;
+  register value $y_301;
+  register value $y_302;
+  register value $y_303;
+  register value $y_304;
+  register value $y_305;
+  register value $y_306;
+  register value $y_307;
+  register value $y_308;
+  register value $y_309;
+  register value $y_310;
+  register value $y_311;
+  register value $y_312;
+  register value $y_313;
+  register value $y_314;
+  register value $y_315;
+  register value $y_316;
+  register value $y_317;
+  register value $y_318;
+  register value $y_319;
+  register value $y_320;
+  register value $y_321;
+  register value $y_322;
+  register value $y_323;
+  register value $y_324;
+  register value $CoqdNumbersdCyclicdInt63dUint63dsize_325;
+  register value $y_327;
+  register value $y_328;
+  register value $y_330;
+  register value $y_332;
+  register value $y_333;
+  register value $y_334;
+  register value $y_335;
+  register value $y_337;
+  register value $CertiCoqdBenchmarksdFibonaccidfibdprogram_339;
+  register value *$alloc;
+  register value *$limit;
+  register value *$args;
+  $alloc = (*$tinfo).alloc;
+  $limit = (*$tinfo).limit;
+  $args = (*$tinfo).args;
+  frame.next = root;
+  frame.root = root;
+  frame.prev = (*$tinfo).fp;
+  if (!(126LL <= $limit - $alloc)) {
+    /*skip*/;
+    (*$tinfo).nalloc = 126LL;
+    garbage_collect($tinfo);
+    /*skip*/;
+    $alloc = (*$tinfo).alloc;
+    $limit = (*$tinfo).limit;
+  }
+  $y_262 = 1LL;
+  $y_263 = (value) ($alloc + 1LL);
+  $alloc = $alloc + 2LL;
+  *((value *) $y_263 + -1LL) = 1024LL;
+  *((value *) $y_263 + 0LL) = $y_262;
+  $y_264 = (value) ($alloc + 1LL);
+  $alloc = $alloc + 2LL;
+  *((value *) $y_264 + -1LL) = 1024LL;
+  *((value *) $y_264 + 0LL) = $y_263;
+  $y_265 = (value) ($alloc + 1LL);
+  $alloc = $alloc + 2LL;
+  *((value *) $y_265 + -1LL) = 1024LL;
+  *((value *) $y_265 + 0LL) = $y_264;
+  $y_266 = (value) ($alloc + 1LL);
+  $alloc = $alloc + 2LL;
+  *((value *) $y_266 + -1LL) = 1024LL;
+  *((value *) $y_266 + 0LL) = $y_265;
+  $y_267 = (value) ($alloc + 1LL);
+  $alloc = $alloc + 2LL;
+  *((value *) $y_267 + -1LL) = 1024LL;
+  *((value *) $y_267 + 0LL) = $y_266;
+  $y_268 = (value) ($alloc + 1LL);
+  $alloc = $alloc + 2LL;
+  *((value *) $y_268 + -1LL) = 1024LL;
+  *((value *) $y_268 + 0LL) = $y_267;
+  $y_269 = (value) ($alloc + 1LL);
+  $alloc = $alloc + 2LL;
+  *((value *) $y_269 + -1LL) = 1024LL;
+  *((value *) $y_269 + 0LL) = $y_268;
+  $y_270 = (value) ($alloc + 1LL);
+  $alloc = $alloc + 2LL;
+  *((value *) $y_270 + -1LL) = 1024LL;
+  *((value *) $y_270 + 0LL) = $y_269;
+  $y_271 = (value) ($alloc + 1LL);
+  $alloc = $alloc + 2LL;
+  *((value *) $y_271 + -1LL) = 1024LL;
+  *((value *) $y_271 + 0LL) = $y_270;
+  $y_272 = (value) ($alloc + 1LL);
+  $alloc = $alloc + 2LL;
+  *((value *) $y_272 + -1LL) = 1024LL;
+  *((value *) $y_272 + 0LL) = $y_271;
+  $y_273 = (value) ($alloc + 1LL);
+  $alloc = $alloc + 2LL;
+  *((value *) $y_273 + -1LL) = 1024LL;
+  *((value *) $y_273 + 0LL) = $y_272;
+  $y_274 = (value) ($alloc + 1LL);
+  $alloc = $alloc + 2LL;
+  *((value *) $y_274 + -1LL) = 1024LL;
+  *((value *) $y_274 + 0LL) = $y_273;
+  $y_275 = (value) ($alloc + 1LL);
+  $alloc = $alloc + 2LL;
+  *((value *) $y_275 + -1LL) = 1024LL;
+  *((value *) $y_275 + 0LL) = $y_274;
+  $y_276 = (value) ($alloc + 1LL);
+  $alloc = $alloc + 2LL;
+  *((value *) $y_276 + -1LL) = 1024LL;
+  *((value *) $y_276 + 0LL) = $y_275;
+  $y_277 = (value) ($alloc + 1LL);
+  $alloc = $alloc + 2LL;
+  *((value *) $y_277 + -1LL) = 1024LL;
+  *((value *) $y_277 + 0LL) = $y_276;
+  $y_278 = (value) ($alloc + 1LL);
+  $alloc = $alloc + 2LL;
+  *((value *) $y_278 + -1LL) = 1024LL;
+  *((value *) $y_278 + 0LL) = $y_277;
+  $y_279 = (value) ($alloc + 1LL);
+  $alloc = $alloc + 2LL;
+  *((value *) $y_279 + -1LL) = 1024LL;
+  *((value *) $y_279 + 0LL) = $y_278;
+  $y_280 = (value) ($alloc + 1LL);
+  $alloc = $alloc + 2LL;
+  *((value *) $y_280 + -1LL) = 1024LL;
+  *((value *) $y_280 + 0LL) = $y_279;
+  $y_281 = (value) ($alloc + 1LL);
+  $alloc = $alloc + 2LL;
+  *((value *) $y_281 + -1LL) = 1024LL;
+  *((value *) $y_281 + 0LL) = $y_280;
+  $y_282 = (value) ($alloc + 1LL);
+  $alloc = $alloc + 2LL;
+  *((value *) $y_282 + -1LL) = 1024LL;
+  *((value *) $y_282 + 0LL) = $y_281;
+  $y_283 = (value) ($alloc + 1LL);
+  $alloc = $alloc + 2LL;
+  *((value *) $y_283 + -1LL) = 1024LL;
+  *((value *) $y_283 + 0LL) = $y_282;
+  $y_284 = (value) ($alloc + 1LL);
+  $alloc = $alloc + 2LL;
+  *((value *) $y_284 + -1LL) = 1024LL;
+  *((value *) $y_284 + 0LL) = $y_283;
+  $y_285 = (value) ($alloc + 1LL);
+  $alloc = $alloc + 2LL;
+  *((value *) $y_285 + -1LL) = 1024LL;
+  *((value *) $y_285 + 0LL) = $y_284;
+  $y_286 = (value) ($alloc + 1LL);
+  $alloc = $alloc + 2LL;
+  *((value *) $y_286 + -1LL) = 1024LL;
+  *((value *) $y_286 + 0LL) = $y_285;
+  $y_287 = (value) ($alloc + 1LL);
+  $alloc = $alloc + 2LL;
+  *((value *) $y_287 + -1LL) = 1024LL;
+  *((value *) $y_287 + 0LL) = $y_286;
+  $y_288 = (value) ($alloc + 1LL);
+  $alloc = $alloc + 2LL;
+  *((value *) $y_288 + -1LL) = 1024LL;
+  *((value *) $y_288 + 0LL) = $y_287;
+  $y_289 = (value) ($alloc + 1LL);
+  $alloc = $alloc + 2LL;
+  *((value *) $y_289 + -1LL) = 1024LL;
+  *((value *) $y_289 + 0LL) = $y_288;
+  $y_290 = (value) ($alloc + 1LL);
+  $alloc = $alloc + 2LL;
+  *((value *) $y_290 + -1LL) = 1024LL;
+  *((value *) $y_290 + 0LL) = $y_289;
+  $y_291 = (value) ($alloc + 1LL);
+  $alloc = $alloc + 2LL;
+  *((value *) $y_291 + -1LL) = 1024LL;
+  *((value *) $y_291 + 0LL) = $y_290;
+  $y_292 = (value) ($alloc + 1LL);
+  $alloc = $alloc + 2LL;
+  *((value *) $y_292 + -1LL) = 1024LL;
+  *((value *) $y_292 + 0LL) = $y_291;
+  $y_293 = (value) ($alloc + 1LL);
+  $alloc = $alloc + 2LL;
+  *((value *) $y_293 + -1LL) = 1024LL;
+  *((value *) $y_293 + 0LL) = $y_292;
+  $y_294 = (value) ($alloc + 1LL);
+  $alloc = $alloc + 2LL;
+  *((value *) $y_294 + -1LL) = 1024LL;
+  *((value *) $y_294 + 0LL) = $y_293;
+  $y_295 = (value) ($alloc + 1LL);
+  $alloc = $alloc + 2LL;
+  *((value *) $y_295 + -1LL) = 1024LL;
+  *((value *) $y_295 + 0LL) = $y_294;
+  $y_296 = (value) ($alloc + 1LL);
+  $alloc = $alloc + 2LL;
+  *((value *) $y_296 + -1LL) = 1024LL;
+  *((value *) $y_296 + 0LL) = $y_295;
+  $y_297 = (value) ($alloc + 1LL);
+  $alloc = $alloc + 2LL;
+  *((value *) $y_297 + -1LL) = 1024LL;
+  *((value *) $y_297 + 0LL) = $y_296;
+  $y_298 = (value) ($alloc + 1LL);
+  $alloc = $alloc + 2LL;
+  *((value *) $y_298 + -1LL) = 1024LL;
+  *((value *) $y_298 + 0LL) = $y_297;
+  $y_299 = (value) ($alloc + 1LL);
+  $alloc = $alloc + 2LL;
+  *((value *) $y_299 + -1LL) = 1024LL;
+  *((value *) $y_299 + 0LL) = $y_298;
+  $y_300 = (value) ($alloc + 1LL);
+  $alloc = $alloc + 2LL;
+  *((value *) $y_300 + -1LL) = 1024LL;
+  *((value *) $y_300 + 0LL) = $y_299;
+  $y_301 = (value) ($alloc + 1LL);
+  $alloc = $alloc + 2LL;
+  *((value *) $y_301 + -1LL) = 1024LL;
+  *((value *) $y_301 + 0LL) = $y_300;
+  $y_302 = (value) ($alloc + 1LL);
+  $alloc = $alloc + 2LL;
+  *((value *) $y_302 + -1LL) = 1024LL;
+  *((value *) $y_302 + 0LL) = $y_301;
+  $y_303 = (value) ($alloc + 1LL);
+  $alloc = $alloc + 2LL;
+  *((value *) $y_303 + -1LL) = 1024LL;
+  *((value *) $y_303 + 0LL) = $y_302;
+  $y_304 = (value) ($alloc + 1LL);
+  $alloc = $alloc + 2LL;
+  *((value *) $y_304 + -1LL) = 1024LL;
+  *((value *) $y_304 + 0LL) = $y_303;
+  $y_305 = (value) ($alloc + 1LL);
+  $alloc = $alloc + 2LL;
+  *((value *) $y_305 + -1LL) = 1024LL;
+  *((value *) $y_305 + 0LL) = $y_304;
+  $y_306 = (value) ($alloc + 1LL);
+  $alloc = $alloc + 2LL;
+  *((value *) $y_306 + -1LL) = 1024LL;
+  *((value *) $y_306 + 0LL) = $y_305;
+  $y_307 = (value) ($alloc + 1LL);
+  $alloc = $alloc + 2LL;
+  *((value *) $y_307 + -1LL) = 1024LL;
+  *((value *) $y_307 + 0LL) = $y_306;
+  $y_308 = (value) ($alloc + 1LL);
+  $alloc = $alloc + 2LL;
+  *((value *) $y_308 + -1LL) = 1024LL;
+  *((value *) $y_308 + 0LL) = $y_307;
+  $y_309 = (value) ($alloc + 1LL);
+  $alloc = $alloc + 2LL;
+  *((value *) $y_309 + -1LL) = 1024LL;
+  *((value *) $y_309 + 0LL) = $y_308;
+  $y_310 = (value) ($alloc + 1LL);
+  $alloc = $alloc + 2LL;
+  *((value *) $y_310 + -1LL) = 1024LL;
+  *((value *) $y_310 + 0LL) = $y_309;
+  $y_311 = (value) ($alloc + 1LL);
+  $alloc = $alloc + 2LL;
+  *((value *) $y_311 + -1LL) = 1024LL;
+  *((value *) $y_311 + 0LL) = $y_310;
+  $y_312 = (value) ($alloc + 1LL);
+  $alloc = $alloc + 2LL;
+  *((value *) $y_312 + -1LL) = 1024LL;
+  *((value *) $y_312 + 0LL) = $y_311;
+  $y_313 = (value) ($alloc + 1LL);
+  $alloc = $alloc + 2LL;
+  *((value *) $y_313 + -1LL) = 1024LL;
+  *((value *) $y_313 + 0LL) = $y_312;
+  $y_314 = (value) ($alloc + 1LL);
+  $alloc = $alloc + 2LL;
+  *((value *) $y_314 + -1LL) = 1024LL;
+  *((value *) $y_314 + 0LL) = $y_313;
+  $y_315 = (value) ($alloc + 1LL);
+  $alloc = $alloc + 2LL;
+  *((value *) $y_315 + -1LL) = 1024LL;
+  *((value *) $y_315 + 0LL) = $y_314;
+  $y_316 = (value) ($alloc + 1LL);
+  $alloc = $alloc + 2LL;
+  *((value *) $y_316 + -1LL) = 1024LL;
+  *((value *) $y_316 + 0LL) = $y_315;
+  $y_317 = (value) ($alloc + 1LL);
+  $alloc = $alloc + 2LL;
+  *((value *) $y_317 + -1LL) = 1024LL;
+  *((value *) $y_317 + 0LL) = $y_316;
+  $y_318 = (value) ($alloc + 1LL);
+  $alloc = $alloc + 2LL;
+  *((value *) $y_318 + -1LL) = 1024LL;
+  *((value *) $y_318 + 0LL) = $y_317;
+  $y_319 = (value) ($alloc + 1LL);
+  $alloc = $alloc + 2LL;
+  *((value *) $y_319 + -1LL) = 1024LL;
+  *((value *) $y_319 + 0LL) = $y_318;
+  $y_320 = (value) ($alloc + 1LL);
+  $alloc = $alloc + 2LL;
+  *((value *) $y_320 + -1LL) = 1024LL;
+  *((value *) $y_320 + 0LL) = $y_319;
+  $y_321 = (value) ($alloc + 1LL);
+  $alloc = $alloc + 2LL;
+  *((value *) $y_321 + -1LL) = 1024LL;
+  *((value *) $y_321 + 0LL) = $y_320;
+  $y_322 = (value) ($alloc + 1LL);
+  $alloc = $alloc + 2LL;
+  *((value *) $y_322 + -1LL) = 1024LL;
+  *((value *) $y_322 + 0LL) = $y_321;
+  $y_323 = (value) ($alloc + 1LL);
+  $alloc = $alloc + 2LL;
+  *((value *) $y_323 + -1LL) = 1024LL;
+  *((value *) $y_323 + 0LL) = $y_322;
+  $y_324 = (value) ($alloc + 1LL);
+  $alloc = $alloc + 2LL;
+  *((value *) $y_324 + -1LL) = 1024LL;
+  *((value *) $y_324 + 0LL) = $y_323;
+  $CoqdNumbersdCyclicdInt63dUint63dsize_325 = (value) ($alloc + 1LL);
+  $alloc = $alloc + 2LL;
+  *((value *) $CoqdNumbersdCyclicdInt63dUint63dsize_325 + -1LL) = 1024LL;
+  *((value *) $CoqdNumbersdCyclicdInt63dUint63dsize_325 + 0LL) = $y_324;
+  $y_327 = 91LLU;
+  $args = (*$tinfo).args;
+  (*$tinfo).alloc = $alloc;
+  (*$tinfo).limit = $limit;
+  *(root + 0LL) = $CoqdNumbersdCyclicdInt63dUint63dsize_325;
+  frame.next = root + 1LL;
+  (*$tinfo).fp = &frame;
+  $y_328 =
+    ((value (*)(struct thread_info *, value, value)) to_Z_rec_uncurried_known_115)
+    ($tinfo, $y_327, $CoqdNumbersdCyclicdInt63dUint63dsize_325);
+  $alloc = (*$tinfo).alloc;
+  $limit = (*$tinfo).limit;
+  $CoqdNumbersdCyclicdInt63dUint63dsize_325 = *(root + 0LL);
+  (*$tinfo).fp = frame.prev;
+  $args = (*$tinfo).args;
+  (*$tinfo).alloc = $alloc;
+  (*$tinfo).limit = $limit;
+  *(root + 0LL) = $CoqdNumbersdCyclicdInt63dUint63dsize_325;
+  frame.next = root + 1LL;
+  (*$tinfo).fp = &frame;
+  $y_330 =
+    ((value (*)(struct thread_info *, value)) f_case_known_117)
+    ($tinfo, $y_328);
+  $alloc = (*$tinfo).alloc;
+  $limit = (*$tinfo).limit;
+  if (!(2LL <= $limit - $alloc)) {
+    *(root + 1LL) = $y_330;
+    frame.next = root + 2LL;
+    (*$tinfo).nalloc = 2LL;
+    garbage_collect($tinfo);
+    $y_330 = *(root + 1LL);
+    $alloc = (*$tinfo).alloc;
+    $limit = (*$tinfo).limit;
+  }
+  $CoqdNumbersdCyclicdInt63dUint63dsize_325 = *(root + 0LL);
+  (*$tinfo).fp = frame.prev;
+  $y_332 = 1LL;
+  $y_333 = (value) ($alloc + 1LL);
+  $alloc = $alloc + 2LL;
+  *((value *) $y_333 + -1LL) = 1024LL;
+  *((value *) $y_333 + 0LL) = $y_332;
+  $y_334 = 1LL;
+  $args = (*$tinfo).args;
+  (*$tinfo).alloc = $alloc;
+  (*$tinfo).limit = $limit;
+  *(root + 0LL) = $CoqdNumbersdCyclicdInt63dUint63dsize_325;
+  frame.next = root + 1LL;
+  (*$tinfo).fp = &frame;
+  $y_335 =
+    ((value (*)(struct thread_info *, value, value, value)) fib_loop_nat_uncurried_uncurried_known_119)
+    ($tinfo, $y_334, $y_333, $y_330);
+  $alloc = (*$tinfo).alloc;
+  $limit = (*$tinfo).limit;
+  $CoqdNumbersdCyclicdInt63dUint63dsize_325 = *(root + 0LL);
+  (*$tinfo).fp = frame.prev;
+  $args = (*$tinfo).args;
+  (*$tinfo).alloc = $alloc;
+  (*$tinfo).limit = $limit;
+  *(root + 0LL) = $CoqdNumbersdCyclicdInt63dUint63dsize_325;
+  frame.next = root + 1LL;
+  (*$tinfo).fp = &frame;
+  $y_337 =
+    ((value (*)(struct thread_info *, value)) f_case_known_120)
+    ($tinfo, $y_335);
+  $alloc = (*$tinfo).alloc;
+  $limit = (*$tinfo).limit;
+  $CoqdNumbersdCyclicdInt63dUint63dsize_325 = *(root + 0LL);
+  (*$tinfo).fp = frame.prev;
+  $args = (*$tinfo).args;
+  (*$tinfo).alloc = $alloc;
+  (*$tinfo).limit = $limit;
+  /*skip*/;
+  $CertiCoqdBenchmarksdFibonaccidfibdprogram_339 =
+    ((value (*)(struct thread_info *, value, value)) f_case_known_123)
+    ($tinfo, $y_337, $CoqdNumbersdCyclicdInt63dUint63dsize_325);
+  $alloc = (*$tinfo).alloc;
+  $limit = (*$tinfo).limit;
+  /*skip*/;
+  (*$tinfo).alloc = $alloc;
+  (*$tinfo).limit = $limit;
+  return $CertiCoqdBenchmarksdFibonaccidfibdprogram_339;
+}
+
+
+#endif /* CERTICOQ_BENCHMARKS_FIBONACCI_FIB_PROGRAM_C */
