benchmarks/fibonacci/fib_main.c
@@ -1,0 +1,28 @@
+/*
+#include <stdio.h>
+#include <stdint.h>
+
+extern uintptr_t program(void);
+
+static inline long long unbox_i63(uintptr_t v) { return (long long)(v >> 1); }
+
+int main(void) {
+    uintptr_t v = program();
+    printf("program ====> %lld\n", unbox_i63(v));
+    return 0;
+} */
+
+#include <stdio.h>
+#include <stdlib.h>
+#include "gc_stack.h"
+
+extern value body(struct thread_info *);
+extern void print_Coq_Init_Datatypes_nat(value);
+
+int main(int argc, char **argv) {
+  struct thread_info *tinfo = make_tinfo();
+  value v = body(tinfo);
+  print_Coq_Init_Datatypes_nat(v);
+  printf("\n");
+  return 0;
+}
