theories/Codegenllvm/LambdaANF_to_llvm.v
@@ -1,17 +1,27 @@
 Unset Universe Checking.
 
-From Coq Require Import Strings.String BinNums ZArith.
+From Coq Require Import Strings.String BinNums ZArith List FMapAVL Floats.
 From ExtLib Require Import Monads.
 Import MonadNotation.
 
-From CertiCoq.LambdaANF Require Import cps toplevel.
-From CertiCoq.Common    Require Import Common Pipeline_utils.
-From MetaCoq.Utils      Require Import MCString.
+From CertiCoq.LambdaANF Require Import cps toplevel cps_util cps_show.
+From CertiCoq.Common Require Import Common Pipeline_utils compM.
+From MetaCoq.Utils Require Import MCString.
+(* Require Import PTree. *)
+
+(* Vellvm AST *)
 From Vellvm.Syntax Require Import LLVMAst.
 
 Open Scope string_scope.
 Open Scope monad_scope.
 Open Scope Z_scope.
+Require Import compcert.lib.Maps.
+
+(* these definitions were used in the dummy compiler, TODO remove *)
+Definition int_ty : LLVMAst.typ := TYPE_I 64%positive.  (* 64-bit int type *)
+
+Definition const_int (z : Z) : LLVMAst.texp LLVMAst.typ :=
+  (int_ty, EXP_Integer z).
 
 Definition i32_42 : texp typ :=
   (TYPE_I 32%positive, EXP_Integer 42%Z).
@@ -38,17 +48,462 @@ Definition trivial_module_ast
   [ TLE_Definition main_def ].
 
 
+(** on Vellvm, a module is a list of TLEs like functions, globals. **)
+(* list of toplevel entity typ of (entry block, other blocks), each of which has
+type (block, typ) *)
+Module VellvmMod.
+  Definition t : Set :=
+    list (LLVMAst.toplevel_entity
+            LLVMAst.typ
+            (LLVMAst.block LLVMAst.typ * list (LLVMAst.block LLVMAst.typ))).
+End VellvmMod.
+
+(*  Useful definitions from certicoqwasm project *)
+(* 1. *)
+Definition get_ctor_arity (cenv : ctor_env) (t : ctor_tag) :=
+  match M.get t cenv with
+  | Some {| ctor_arity := n |} => Ret (N.to_nat n)
+  | _ => Err "found constructor without ctor_arity set"
+  end.
+
+(* 2. *)
+Definition collect_function_vars (e : cps.exp) : list cps.var :=
+    match e with
+    | Efun fds exp => (* fundefs only allowed here (uppermost level) *)
+      (fix iter (fds : fundefs) : list cps.var :=
+          match fds with
+          | Fnil => []
+          | Fcons x _ _ e' fds' => x :: (iter fds')
+          end) fds
+    | _ => []
+    end.
+
+(* environment that maps LambdaANF variables to llvm identifiers.
+   Kept around for later *)
+Definition local_env := PTree.t raw_id.
+
+(* positive / nat -> stdlib string (the type Vellvm's [Name] expects). The C
+   name in prim_env and MCString produce MetaCoq bytestrings, so, convert. *)
+Definition pos_to_str (p : positive) : String.string :=
+  bytestring.String.to_string (MCString.string_of_positive p).
+Definition nat_to_str (n : nat) : String.string :=
+  bytestring.String.to_string (MCString.string_of_nat n).
+
+(* Map a LambdaANF variable to a *named* Vellvm identifier "%v<n>". *)
+Definition var_to_id (x : var) : raw_id := Name (("v" ++ pos_to_str x)%string).
+
+
+
+(** * Value representation 
+mirrors LambdaANF_to_Clight. 
+Will need to be updated with GC. 
+*)
+
+Definition word_t   : typ := TYPE_I 64%positive.
+Definition wordptr_t : typ := TYPE_Pointer (Some word_t).
+Definition i8_t     : typ := TYPE_I 8%positive.
+Definition i8ptr_t  : typ := TYPE_Pointer (Some i8_t).
+
+Inductive ctor_rep : Set :=
+| rep_enum  (ord : N)            (* unboxed, nullary constructor *)
+| rep_boxed (ord : N) (arity : N). (* boxed, arity > 0 *)
+
+Definition get_ctor_rep (cenv : ctor_env) (t : ctor_tag) : error ctor_rep :=
+  match M.get t cenv with
+  | Some info =>
+      if (ctor_arity info =? 0)%N
+      then Ret (rep_enum (ctor_ordinal info))
+      else Ret (rep_boxed (ctor_ordinal info) (ctor_arity info))
+  | None => Err "get_ctor_rep: constructor tag not found in ctor_env"
+  end.
+
+Definition enum_immediate (ord : N) : Z := (Z.shiftl (Z.of_N ord) 1 + 1)%Z.
+Definition boxed_header (ord arity : N) : Z := (Z.shiftl (Z.of_N arity) 10 + Z.of_N ord)%Z.
+
+(* CertiCoq's boxed-float header tag  *)
+Definition float_header : Z := 1277%Z.
+
+
+Definition f64_join_bits (s : bool) (m e : Z) : Z :=
+  (Z.shiftl ((if s then Z.pow 2 11 else 0) + e) 52 + m)%Z.
+
+Definition bits_of_spec_float (x : SpecFloat.spec_float) : Z :=
+  match x with
+  | SpecFloat.S754_zero s       => f64_join_bits s 0 0
+  | SpecFloat.S754_infinity s   => f64_join_bits s 0 (Z.pow 2 11 - 1)
+  | SpecFloat.S754_nan          => f64_join_bits false (Z.pow 2 51) (Z.pow 2 11 - 1)
+  | SpecFloat.S754_finite s m e =>
+      let mm := (Z.pos m - Z.pow 2 52)%Z in
+      if Z.leb 0 mm
+      then f64_join_bits s mm (e + 1075)     (* normalized: e - emin + 1 *)
+      else f64_join_bits s (Z.pos m) 0       
+  end.
+
+Definition float_to_bits (f : PrimFloat.float) : Z :=
+  bits_of_spec_float (FloatOps.Prim2SF f).
+
+(* the i64 operand holding the value of a LambdaANF variable *)
+Definition var_operand (x : var) : texp typ := (word_t, EXP_Ident (ID_Local (var_to_id x))).
+
+
+Definition cg_code := list (instr_id * instr typ).
+
+
+Definition genM (A : Type) : Type := Z -> error (A * cg_code * list (block typ) * Z).
+
+Definition gen_ret {A} (a : A) : genM A := fun s => Ret (a, [], [], s).
+
+Definition gen_bind {A B} (m : genM A) (f : A -> genM B) : genM B :=
+  fun s =>
+    match m s with
+    | Err e => Err e
+    | Ret (a, c1, b1, s1) =>
+        match f a s1 with
+        | Err e => Err e
+        | Ret (b, c2, b2, s2) => Ret (b, (c1 ++ c2)%list, (b1 ++ b2)%list, s2)
+        end
+    end.
+
+#[global] Instance Monad_genM : Monad genM :=
+  { ret := @gen_ret ; bind := @gen_bind }.
+
+Definition gen_fail {A} (msg : string) : genM A := fun _ => Err msg.
+
+Definition lift_err {A} (e : error A) : genM A :=
+  fun s => match e with Ret a => Ret (a, [], [], s) | Err m => Err m end.
+
+(* fresh named SSA id "%t<n>" for an intermediate value or a block label;
+   disjoint from source variables' "%v<n>" ids (see [var_to_id]) *)
+Definition fresh_id : genM raw_id :=
+  fun s => Ret (Name (("t" ++ nat_to_str (Z.to_nat s))%string), [], [], (s + 1)%Z).
+(* fresh number for a void instruction id (store) *)
+Definition fresh_void : genM int_ast := fun s => Ret (s, [], [], (s + 1)%Z).
+
+Definition emit (i : instr_id * instr typ) : genM Datatypes.unit := fun s => Ret (tt, [i], [], s).
+
+(* add an already-completed basic block to the output *)
+Definition emit_block (b : block typ) : genM Datatypes.unit := fun s => Ret (tt, [], [b], s).
+
+(* run [m] but return its current-block code instead of merging it into the
+   surrounding block; completed blocks and the counter still propagate. Used to
+   collect the body of an Ecase arm into its own block. *)
+Definition capture {A} (m : genM A) : genM (cg_code * A) :=
+  fun s =>
+    match m s with
+    | Err e => Err e
+    | Ret (a, code, blks, s') => Ret ((code, a), [], blks, s')
+    end.
+
+(* emit an operation producing a fresh local; return its operand expression *)
+Definition emit_op (op : exp typ) : genM (exp typ) :=
+  id <- fresh_id ;;
+  emit (IId id, INSTR_Op op) ;;
+  ret (EXP_Ident (ID_Local id)).
+
+(* bind a LambdaANF variable [x] to the result of operation [op] *)
+Definition bind_var_op (x : var) (op : exp typ) : genM Datatypes.unit :=
+  emit (IId (var_to_id x), INSTR_Op op).
+
+Definition malloc_fn : texp typ :=
+  (i8ptr_t, EXP_Ident (ID_Global (Name "malloc"))).
+
+(* Build a function declaration with empty per-argument attributes. ShowAST
+   requires the args-attrs list to have exactly one entry per argument (it
+  combines them, and the definition printer errors on a length mismatch). *)
+Definition mk_fun_decl (name : raw_id) (ret : typ) (argtys : list typ) : declaration typ :=
+  mk_declaration name (TYPE_Function ret argtys false)
+                 ([], List.repeat (@nil param_attr) (List.length argtys)) [] [].
+
+Definition malloc_decl : declaration typ :=
+  mk_fun_decl (Name "malloc") i8ptr_t [word_t].
+
+(* call malloc for [nbytes] and return the i64* base pointer *)
+Definition gen_alloc (nbytes : Z) : genM (exp typ) :=
+  raw  <- (id <- fresh_id ;;
+           emit (IId id, INSTR_Call malloc_fn [((word_t, EXP_Integer nbytes), [])] []) ;;
+           ret (EXP_Ident (ID_Local id))) ;;
+  emit_op (OP_Conversion Bitcast i8ptr_t raw wordptr_t).
+
+(* store [val] at i64* [ptr] *)
+Definition gen_store (ptr : exp typ) (val : texp typ) : genM Datatypes.unit :=
+  n <- fresh_void ;;
+  emit (IVoid n, INSTR_Store val (wordptr_t, ptr) []).
+
+(* getelementptr i64, i64* [ptr], i64 [i] -> i64* to element [i] *)
+Definition gen_gep (ptr : exp typ) (i : Z) : genM (exp typ) :=
+  emit_op (OP_GetElementPtr word_t (wordptr_t, ptr) [(word_t, EXP_Integer i)]).
+
+(* is [v] one of the top-level function names? *)
+Definition is_fname (fnames : list var) (v : var) : bool :=
+  List.existsb (fun g => Pos.eqb g v) fnames.
+
+
+Definition gen_operand (fnames : list var) (y : var) : genM (texp typ) :=
+  if is_fname fnames y
+  then addr <- emit_op (OP_Conversion Ptrtoint wordptr_t
+                          (EXP_Ident (ID_Global (var_to_id y))) word_t) ;;
+       ret (word_t, addr)
+  else ret (var_operand y).
+
+(* store the fields [ys] starting at field-pointer [fieldptr], index [i] *)
+Fixpoint store_fields (fnames : list var) (fieldptr : exp typ) (i : Z) (ys : list var) : genM Datatypes.unit :=
+  match ys with
+  | [] => ret tt
+  | y :: ys' =>
+      slot <- gen_gep fieldptr i ;;
+      v    <- gen_operand fnames y ;;
+      gen_store slot v ;;
+      store_fields fnames fieldptr (i + 1) ys'
+  end.
+
+
+Fixpoint gen_args (fnames : list var) (ys : list var)
+  : genM (list (texp typ * list param_attr)) :=
+  match ys with
+  | [] => ret []
+  | y :: ys' =>
+      v    <- gen_operand fnames y ;;
+      rest <- gen_args fnames ys' ;;
+      ret ((v, @nil param_attr) :: rest)
+  end.
+
+(* the callee operand for applying [f] to [nargs] arguments *)
+Definition gen_callee (fnames : list var) (f : var) (nargs : nat) : genM (texp typ) :=
+  if is_fname fnames f
+  then 
+    ret (word_t, EXP_Ident (ID_Global (var_to_id f)))
+  else (* indirect call: f is an i64 word holding a function pointer *)
+    let fnty := TYPE_Function word_t (List.repeat word_t nargs) false in
+    fp <- emit_op (OP_Conversion Inttoptr word_t (EXP_Ident (ID_Local (var_to_id f)))
+                                 (TYPE_Pointer (Some fnty))) ;;
+    ret (word_t, fp).
+
+Definition switch_case (ord : N) (lbl : block_id) : tint_literal * block_id :=
+  (TInt_Literal 64%positive (Z.of_N ord), lbl).
+
+(* NOTE: [exp] is qualified as [cps.exp]; importing Vellvm's LLVMAst shadows the
+   bare [exp] with the LLVM expression type ([exp : Set -> Set]).
+    *)
+Fixpoint translate_exp (cenv : ctor_env) (penv : prim_env) (fnames : list var) (e : cps.exp) : genM (terminator typ) :=
+  match e with
+  | Ehalt x =>
+      op <- gen_operand fnames x ;;
+      ret (TERM_Ret op)
+  | Econstr x t ys e' =>
+      rep <- lift_err (get_ctor_rep cenv t) ;;
+      match rep with
+      | rep_enum ord =>
+          (* x := (ord << 1) + 1, materialized as an i64 SSA value *)
+          bind_var_op x (OP_IBinop Or word_t (EXP_Integer (enum_immediate ord)) (EXP_Integer 0%Z)) ;;
+          translate_exp cenv penv fnames e'
+      | rep_boxed ord arity =>
+          base     <- gen_alloc ((Z.of_N arity + 1) * 8) ;;               (* header + fields *)
+          gen_store base (word_t, EXP_Integer (boxed_header ord arity)) ;; (* header at base[0] *)
+          fieldptr <- gen_gep base 1 ;;                                    (* pointer to field 0 *)
+          store_fields fnames fieldptr 0 ys ;;
+          (* the value word of x is the field pointer, as an integer *)
+          bind_var_op x (OP_Conversion Ptrtoint wordptr_t fieldptr word_t) ;;
+          translate_exp cenv penv fnames e'
+      end
+  | Eproj x t n y e' =>
+      (* x := y[n]; y is a boxed pointer (points at field 0) *)
+      yptr <- emit_op (OP_Conversion Inttoptr word_t (EXP_Ident (ID_Local (var_to_id y))) wordptr_t) ;;
+      slot <- gen_gep yptr (Z.of_N n) ;;
+      emit (IId (var_to_id x), INSTR_Load word_t (wordptr_t, slot) []) ;;
+      translate_exp cenv penv fnames e'
+  | Eapp f t ys =>
+      (* tail call: %r = call f(ys); ret %r *)
+      callee <- gen_callee fnames f (List.length ys) ;;
+      args <- gen_args fnames ys ;;
+      r <- (id <- fresh_id ;;
+            emit (IId id, INSTR_Call callee args []) ;;
+            ret (EXP_Ident (ID_Local id))) ;;
+      ret (TERM_Ret (word_t, r))
+  | Eletapp x f t ys e' =>
+      (* non-tail call: %x = call f(ys); continue *)
+      callee <- gen_callee fnames f (List.length ys) ;;
+      args <- gen_args fnames ys ;;
+      emit (IId (var_to_id x), INSTR_Call callee args []) ;;
+      translate_exp cenv penv fnames e'
+  | Ecase y arms =>
+      let fix gen_arms (arms : list (ctor_tag * cps.exp))
+          : genM (list (ctor_rep * block_id)) :=
+          match arms with
+          | [] => ret []
+          | (ct, ei) :: rest =>
+              rep <- lift_err (get_ctor_rep cenv ct) ;;
+              lbl <- fresh_id ;;
+              cap <- capture (translate_exp cenv penv fnames ei) ;;
+              let '(code, term) := cap in
+              emit_block (mk_block lbl [] code term None) ;;
+              rest' <- gen_arms rest ;;
+              ret ((rep, lbl) :: rest')
+          end in
+      classified <- gen_arms arms ;;
+      let yval := EXP_Ident (ID_Local (var_to_id y)) in
+      let unboxed_cases :=
+        List.flat_map (fun rl => match rl with
+                                 | (rep_enum o, l) => [switch_case o l]
+                                 | _ => [] end) classified in
+      let boxed_cases :=
+        List.flat_map (fun rl => match rl with
+                                 | (rep_boxed o _, l) => [switch_case o l]
+                                 | _ => [] end) classified in
+      ub_lbl  <- fresh_id ;;
+      bx_lbl  <- fresh_id ;;
+      def_lbl <- fresh_id ;;
+      emit_block (mk_block def_lbl [] [] TERM_Unreachable None) ;;
+      (* unboxed dispatch: switch on (y >> 1) *)
+      ordu <- fresh_id ;;
+      emit_block (mk_block ub_lbl []
+        [(IId ordu, INSTR_Op (OP_IBinop (LShr false) word_t yval (EXP_Integer 1%Z)))]
+        (TERM_Switch (word_t, EXP_Ident (ID_Local ordu)) def_lbl unboxed_cases) None) ;;
+      (* boxed dispatch: header at y[-1], switch on (header & 255) *)
+      hp    <- fresh_id ;;
+      hslot <- fresh_id ;;
+      hdr   <- fresh_id ;;
+      ordb  <- fresh_id ;;
+      emit_block (mk_block bx_lbl []
+        [ (IId hp,    INSTR_Op (OP_Conversion Inttoptr word_t yval wordptr_t))
+        ; (IId hslot, INSTR_Op (OP_GetElementPtr word_t (wordptr_t, EXP_Ident (ID_Local hp))
+                                                 [(word_t, EXP_Integer (-1)%Z)]))
+        ; (IId hdr,   INSTR_Load word_t (wordptr_t, EXP_Ident (ID_Local hslot)) [])
+        ; (IId ordb,  INSTR_Op (OP_IBinop And word_t (EXP_Ident (ID_Local hdr)) (EXP_Integer 255%Z)))
+        ]
+        (TERM_Switch (word_t, EXP_Ident (ID_Local ordb)) def_lbl boxed_cases) None) ;;
+      (* current block: test low bit, branch to the matching dispatch block *)
+      lb  <- fresh_id ;;
+      emit (IId lb, INSTR_Op (OP_IBinop And word_t yval (EXP_Integer 1%Z))) ;;
+      isu <- fresh_id ;;
+      emit (IId isu, INSTR_Op (OP_ICmp Eq word_t (EXP_Ident (ID_Local lb)) (EXP_Integer 1%Z))) ;;
+      ret (TERM_Br (TYPE_I 1%positive, EXP_Ident (ID_Local isu)) ub_lbl bx_lbl)
+  | Efun _ _ =>
+         which also rejects Efun inside a body) *)
+      gen_fail "translate_exp: nested Efun (term should be hoisted)"
+  | Eprim_val x p e' =>
+      match p with
+      | existT AstCommon.primInt i =>
+          (* unboxed primitive int: x := 2 * to_Z(i) + 1 (same tagging as enum) *)
+          bind_var_op x (OP_IBinop Or word_t
+                          (EXP_Integer (2 * Uint63.to_Z i + 1)%Z) (EXP_Integer 0%Z)) ;;
+          translate_exp cenv penv fnames e'
+      | existT AstCommon.primFloat f =>
+          (* boxed float: 2 words = header [1277] + the 64-bit pattern; x points
+             at field 0 (header at x[-1]), same layout as a boxed constructor. *)
+          base     <- gen_alloc (2 * 8) ;;
+          gen_store base (word_t, EXP_Integer float_header) ;;
+          fieldptr <- gen_gep base 1 ;;
+          gen_store fieldptr (word_t, EXP_Integer (float_to_bits f)) ;;
+          bind_var_op x (OP_Conversion Ptrtoint wordptr_t fieldptr word_t) ;;
+          translate_exp cenv penv fnames e'
+      end
+  | Eprim x p ys e' =>
+      (* apply an external primitive operator, resolved by C name via prim_env *)
+      match M.get p penv with
+      | None => gen_fail "translate_exp: Eprim primitive id not found in prim_env"
+      | Some (_, cname, tinfo, _) =>
+          if tinfo
+          then gen_fail "translate_exp: Eprim with tinfo unsupported in no-GC backend"
+          else
+            let callee : texp typ :=
+              (word_t, EXP_Ident (ID_Global (Name (bytestring.String.to_string cname)))) in
+            args <- gen_args fnames ys ;;
+            emit (IId (var_to_id x), INSTR_Call callee args []) ;;
+            translate_exp cenv penv fnames e'
+      end
+  end.
+
+(** ** Assembling functions and the whole program *)
+
+(* run the body translator and wrap the result into a single entry block *)
+Definition translate_exp_to_block (cenv : ctor_env) (penv : prim_env) (fnames : list var) (e : cps.exp)
+  : error (block typ * list (block typ)) :=
+  match translate_exp cenv penv fnames e 0%Z with
+  | Err m => Err m
+  | Ret (term, code, blks, _) => Ret (mk_block (Name "entry") [] code term None, blks)
+  end.
+
+(* a function definition returning i64 and taking params as i64 words *)
+Definition mk_fn_def (name : raw_id) (params : list var)
+                     (instrs : block typ * list (block typ))
+  : definition typ (block typ * list (block typ)) :=
+  let argtys := List.map (fun _ => word_t) params in
+  {| df_prototype := mk_fun_decl name word_t argtys
+   ; df_args      := List.map var_to_id params
+   ; df_instrs    := instrs
+  |}.
+
+(* the entry point: main () -> i64 *)
+Definition mk_main_def (instrs : block typ * list (block typ))
+  : definition typ (block typ * list (block typ)) :=
+  {| df_prototype := mk_fun_decl (Name "main") word_t []
+   ; df_args      := []
+   ; df_instrs    := instrs
+  |}.
+
+(* translate the top-level function definitions *)
+Fixpoint translate_fundefs (cenv : ctor_env) (penv : prim_env) (fnames : list var) (fds : fundefs)
+  : error (list (toplevel_entity typ (block typ * list (block typ)))) :=
+  match fds with
+  | Fnil => Ret []
+  | Fcons f t params body fds' =>
+      match translate_exp_to_block cenv penv fnames body with
+      | Err m => Err m
+      | Ret instrs =>
+          match translate_fundefs cenv penv fnames fds' with
+          | Err m => Err m
+          | Ret rest => Ret (TLE_Definition (mk_fn_def (var_to_id f) params instrs) :: rest)
+          end
+      end
+  end.
+
+Definition prim_decls (penv : prim_env)
+  : list (toplevel_entity typ (block typ * list (block typ))) :=
+  List.map (fun kv =>
+              let '(_, (_, cname, _, ar)) := kv in
+              TLE_Declaration (mk_fun_decl (Name (bytestring.String.to_string cname))
+                                           word_t (List.repeat word_t ar)))
+           (M.elements penv).
+
+Definition translate_program (cenv : ctor_env) (penv : prim_env) (prog : cps.exp)
+  : error (list (toplevel_entity typ (block typ * list (block typ)))) :=
+  let fnames := collect_function_vars prog in
+  let externs := TLE_Declaration malloc_decl :: prim_decls penv in
+  match prog with
+  | Efun fds e =>
+      match translate_fundefs cenv penv fnames fds with
+      | Err m => Err m
+      | Ret fdefs =>
+          match translate_exp_to_block cenv penv fnames e with
+          | Err m => Err m
+          | Ret instrs =>
+              Ret (externs ++ fdefs ++ [TLE_Definition (mk_main_def instrs)])%list
+          end
+      end
+  | _ =>
+      match translate_exp_to_block cenv penv fnames prog with
+      | Err m => Err m
+      | Ret instrs =>
+          Ret (externs ++ [TLE_Definition (mk_main_def instrs)])%list
+      end
+  end.
+
+
+
 
 Definition compile_LambdaANF_to_llvm
   (prims : list (kername * string * bool * nat * positive))
   : CertiCoqTrans toplevel.LambdaANF_FullTerm
                   (list (toplevel_entity typ (block typ * list (block typ)))) :=
   fun st =>
-    debug_msg "Translating LambdaANF to Vellvm AST (dummy i32 42)" ;;
+    debug_msg "Translating LambdaANF to Vellvm AST" ;;
     _opts <- get_options ;;
     LiftErrorCertiCoqTrans
       "CodegenLLVM(AST)"
-      (fun '(_env, _e) =>
-         (* TODO: translate (_env, _e) after dummy compiler *)
-         compM.Ret trivial_module_ast)
+      (fun '(env, prog) =>
+         let '(_pr, penv, cenv, _ctag, _itag, _nenv, _fenv, _rho) := env in
+         match translate_program cenv penv prog with
+         | Err msg => compM.Err msg
+         | Ret tles => compM.Ret tles
+         end)
       st.
