benchmarks/fibonacci/fib.v
@@ -1,0 +1,35 @@
+From Coq Require Import Uint63 ZArith.
+
+Open Scope uint63_scope.
+
+(* nat-iterative Fibonacci *)
+Fixpoint fib_loop_nat (i a b : nat) : nat :=
+  match i with
+  | 0%nat => b
+  | S i'  => fib_loop_nat i' (a + b)%nat a
+  end.
+
+Definition fib_nat (n : nat) : nat :=
+  fib_loop_nat n 1%nat 0%nat.
+
+Definition int_to_nat (x : int) : nat :=
+  Z.to_nat (Uint63.to_Z x).
+
+Definition nat_to_int (n : nat) : int :=
+  Uint63.of_Z (Z.of_nat n).
+
+Definition fib63 (n : int) : int :=
+  nat_to_int (fib_nat (int_to_nat n)).
+
+Definition program : int := fib63 45%uint63.
+
+From CertiCoq.Plugin Require Import CertiCoq.
+(* CertiCoq Compile program.*)
+
+(* CertiCoq Run -build_dir "extraction" program. *)
+
+CertiCoq Compile -build_dir "extraction" program.
+
+(* CertiCoq Compile -config 1 -0 1 -ext "_fib1" program. *)
+
+CertiCoq Generate Glue -file "glue_fib" [ nat ].
