theories/Codegenllvm/tests/test_basic.v
@@ -1,0 +1,36 @@
+Unset Universe Checking.
+
+From Coq Require Import List ZArith Strings.String.
+From CertiCoq.LambdaANF Require Import cps toplevel.
+From CertiCoq.Common Require Import Common compM.
+From CertiCoq.Codegenllvm Require Import LambdaANF_to_llvm.
+From Vellvm.QC Require Import ShowAST.
+From Vellvm.Syntax Require Import LLVMAst.
+Import ListNotations.
+
+
+Definition cenv : ctor_env :=
+  M.set 10%positive (Build_ctor_ty_info nAnon nAnon 1%positive 0%N 0%N)
+ (M.set 11%positive (Build_ctor_ty_info nAnon nAnon 1%positive 2%N 0%N)
+ (M.empty _)).
+
+Definition penv : prim_env := M.empty _.
+
+
+Definition run (e : cps.exp) : String.string :=
+  match translate_program cenv penv e with
+  | Ret m => showProg m
+  | Err _ => "translate_program returned Err"%string
+  end.
+
+
+Definition t_enum : cps.exp :=
+  Econstr 1%positive 10%positive [] (Ehalt 1%positive).
+Eval vm_compute in (run t_enum).
+
+Definition t_boxed : cps.exp :=
+  Econstr 1%positive 10%positive []
+    (Econstr 2%positive 11%positive [1%positive; 1%positive]
+      (Eproj 3%positive 11%positive 0%N 2%positive
+        (Ehalt 3%positive))).
+Eval vm_compute in (run t_boxed).
