theories/Codegenllvm/tests/test_basic2.v
@@ -1,0 +1,51 @@
+Unset Universe Checking.
+
+From Coq Require Import List ZArith Strings.String.
+From CertiCoq.LambdaANF Require Import cps toplevel.
+From CertiCoq.Common Require Import Common compM.
+From CertiCoq.Codegenllvm Require Import LambdaANF_to_llvm.
+From Vellvm.QC Require Import ShowAST.
+From Vellvm.Syntax Require Import LLVMAst.
+Import ListNotations.
+
+Definition mkc (arity ord : N) : ctor_ty_info :=
+  Build_ctor_ty_info nAnon nAnon 1%positive arity ord.
+
+Definition cenv : ctor_env :=
+  M.set 10%positive (mkc 0 0)
+ (M.set 11%positive (mkc 2 0)
+ (M.set 30%positive (mkc 0 0)
+ (M.set 31%positive (mkc 0 1)
+ (M.set 40%positive (mkc 0 5)
+ (M.set 41%positive (mkc 0 7)
+ (M.empty _)))))).
+
+Definition penv : prim_env := M.empty _.
+
+Definition run (e : cps.exp) : String.string :=
+  match translate_program cenv penv e with
+  | Ret m => showProg m
+  | Err _ => "translate_program returned Err"%string
+  end.
+
+
+Definition t_case_unboxed : cps.exp :=
+  Econstr 1%positive 31%positive []
+    (Ecase 1%positive
+      [ (30%positive, Econstr 2%positive 40%positive [] (Ehalt 2%positive))
+      ; (31%positive, Econstr 3%positive 41%positive [] (Ehalt 3%positive)) ]).
+Eval vm_compute in (run t_case_unboxed).
+
+
+Definition t_case_boxed : cps.exp :=
+  Econstr 1%positive 10%positive []
+    (Econstr 2%positive 11%positive [1%positive; 1%positive]
+      (Ecase 2%positive
+        [ (11%positive, Eproj 3%positive 11%positive 0%N 2%positive (Ehalt 3%positive)) ])).
+Eval vm_compute in (run t_case_boxed).
+
+
+Definition t_fun : cps.exp :=
+  Efun (Fcons 5%positive 1%positive [6%positive] (Ehalt 6%positive) Fnil)
+    (Econstr 1%positive 10%positive [] (Eapp 5%positive 1%positive [1%positive])).
+Eval vm_compute in (run t_fun).
