theories/Codegenllvm/tests/test_basic3.v
@@ -1,0 +1,48 @@
+Unset Universe Checking.
+
+From Coq Require Import List ZArith Strings.String.
+From CertiCoq.LambdaANF Require Import cps toplevel.
+From CertiCoq.Common Require Import Common compM.
+From CertiCoq.Codegenllvm Require Import LambdaANF_to_llvm.
+From Vellvm.QC Require Import ShowAST.
+From Vellvm.Syntax Require Import LLVMAst.
+Import ListNotations.
+
+Definition mkc (arity ord : N) : ctor_ty_info :=
+  Build_ctor_ty_info nAnon nAnon 1%positive arity ord.
+
+
+Definition cenv : ctor_env :=
+  M.set 10%positive (mkc 0 0)
+ (M.set 31%positive (mkc 0 1)
+ (M.set 11%positive (mkc 2 0)
+ (M.set 12%positive (mkc 1 0)
+ (M.empty _)))).
+
+Definition penv : prim_env := M.empty _.
+
+Definition run (e : cps.exp) : String.string :=
+  match translate_program cenv penv e with
+  | Ret m => showProg m
+  | Err _ => "translate_program returned Err"%string
+  end.
+
+
+Definition t_field1 : cps.exp :=
+  Econstr 1%positive 10%positive []
+    (Econstr 2%positive 31%positive []
+      (Econstr 3%positive 11%positive [1%positive; 2%positive]
+        (Eproj 4%positive 11%positive 1%N 3%positive
+          (Ehalt 4%positive)))).
+Eval vm_compute in (run t_field1).
+
+
+Definition t_nested : cps.exp :=
+  Econstr 1%positive 10%positive []
+    (Econstr 2%positive 31%positive []
+      (Econstr 3%positive 11%positive [1%positive; 2%positive]
+        (Econstr 4%positive 12%positive [3%positive]
+          (Eproj 5%positive 12%positive 0%N 4%positive
+            (Eproj 6%positive 11%positive 1%N 5%positive
+              (Ehalt 6%positive)))))).
+Eval vm_compute in (run t_nested).
