theories/Codegenllvm/tests/test_basic4.v
@@ -1,0 +1,34 @@
+Unset Universe Checking.
+
+From Coq Require Import List ZArith Strings.String.
+From CertiCoq.LambdaANF Require Import cps toplevel.
+From CertiCoq.Common Require Import Common compM.
+From CertiCoq.Codegenllvm Require Import LambdaANF_to_llvm.
+From Vellvm.QC Require Import ShowAST.
+From Vellvm.Syntax Require Import LLVMAst.
+Import ListNotations.
+
+Definition mkc (arity ord : N) : ctor_ty_info :=
+  Build_ctor_ty_info nAnon nAnon 1%positive arity ord.
+
+Definition cenv : ctor_env :=
+  M.set 10%positive (mkc 0 0) (M.empty _).   (* enum ctor, value 1 *)
+
+Definition penv : prim_env := M.empty _.
+
+Definition run (e : cps.exp) : String.string :=
+  match translate_program cenv penv e with
+  | Ret m => showProg m
+  | Err _ => "translate_program returned Err"%string
+  end.
+
+
+Definition t_indirect : cps.exp :=
+  Efun
+    (Fcons 100%positive 1%positive [101%positive] (Ehalt 101%positive)
+      (Fcons 102%positive 1%positive [103%positive]
+        (Econstr 104%positive 10%positive []
+          (Eapp 103%positive 1%positive [104%positive]))
+        Fnil))
+    (Eapp 102%positive 1%positive [100%positive]).
+Eval vm_compute in (run t_indirect).
