theories/Codegenllvm/tests/test_basic5.v
@@ -1,0 +1,26 @@
+Unset Universe Checking.
+
+From Coq Require Import List ZArith Strings.String Floats.
+From CertiCoq.LambdaANF Require Import cps toplevel.
+From CertiCoq.Common Require Import Common compM AstCommon.
+From CertiCoq.Codegenllvm Require Import LambdaANF_to_llvm.
+From Vellvm.QC Require Import ShowAST.
+From Vellvm.Syntax Require Import LLVMAst.
+Import ListNotations.
+
+Definition cenv : ctor_env := M.empty _.   (* unused: Eproj/Eprim_val need no ctor info *)
+Definition penv : prim_env := M.empty _.
+
+Definition run (e : cps.exp) : String.string :=
+  match translate_program cenv penv e with
+  | Ret m => showProg m
+  | Err _ => "translate_program returned Err"%string
+  end.
+
+Eval vm_compute in (float_to_bits 1.5%float).
+
+Definition t_float : cps.exp :=
+  Eprim_val 1%positive (existT AstCommon.prim_value AstCommon.primFloat 1.5%float)
+    (Eproj 2%positive 1%positive 0%N 1%positive
+      (Ehalt 2%positive)).
+Eval vm_compute in (run t_float).
